Checking in various stuff. I haven't finished the main result I'm trying to prove (correctness of clock implementation rewrites), but have made substantial progress thanks to help from the IBM folks.

examples/Sugar2/Sugar2Script.sml
@@ -1,5 +1,7 @@
+
 (*****************************************************************************)
 (* Some sanity checking properties of the Sugar 2.0 semantics in HOL         *)
+(* This is a working file, so contains lots of unused and useless stuff      *)
 (*****************************************************************************)
 
 (*****************************************************************************)
@@ -12,7 +14,8 @@
 ******************************************************************************)
 (*
 load "Sugar2SemanticsTheory"; 
-load "rich_listTheory"; load "intLib"; load "res_quanTheory";
+load "rich_listTheory"; load "intLib"; 
+load "res_quanLib";load "res_quanTheory";
 
 quietdec := true;
 open Sugar2SemanticsTheory PathTheory 
@@ -39,6 +42,15 @@ open Sugar2SemanticsTheory PathTheory
 * Set default parsing to natural numbers rather than integers 
 ******************************************************************************)
 val _ = intLib.deprecate_int();
+
+val resd = 
+ simpLib.SIMPSET {ac = [], congs = [],
+                  convs = 
+                   [{conv = K (K (res_quanLib.RES_FORALL_CONV 
+                                  ORELSEC res_quanLib.RES_EXISTS_CONV)),
+                    key = SOME([],``(P:('a -> bool) -> ('a -> bool) -> bool)(\x. Q x)``), 
+                    name = "RES_CONV", trace = 2}],
+                    dprocs = [], filter = NONE, rewrs = []};
 
 (******************************************************************************
 * Start a new theory called Sugar2
@@ -418,6 +430,39 @@ val NEXT_RISE_LEQ_TRUE_EXISTS =
     THEN RW_TAC arith_ss 
      [SIMP_RULE arith_ss [] (Q.SPECL[`p`,`j`,`j`](GEN_ALL NEXT_RISE_TRUE))]);
 
+val NEXT_RISE_LESS =
+ store_thm
+  ("NEXT_RISE_LESS",
+   ``i <= j /\ NEXT_RISE M p c (i,j) =
+      i <= j 
+      /\
+      (!k. i <= k /\ k < j ==> ~B_SEM M (getL M (PATH_EL p k)) c) 
+      /\
+      B_SEM M (getL M (PATH_EL p j)) c``,
+   PROVE_TAC[NEXT_RISE]);
+
+val FIRST_RISE_RESTN =
+ store_thm
+  ("FIRST_RISE_RESTN",
+   ``!i j. FIRST_RISE M (RESTN p i) c j = NEXT_RISE M p c (i,i+j)``,
+   Induct
+    THEN RW_TAC arith_ss [FIRST_RISE, NEXT_RISE, RESTN_def,PATH_EL_RESTN]
+    THEN EQ_TAC
+    THEN RW_TAC arith_ss []
+    THEN `k - SUC i < j` by DECIDE_TAC
+    THEN `(k - SUC i) + SUC i = k` by DECIDE_TAC
+    THEN PROVE_TAC[]);
+
+val NEXT_RISE_FIRST_RISE =
+ store_thm
+  ("FIRST_RISE_RESTN",
+   ``!i j. i <= j 
+           ==> 
+           (NEXT_RISE M p c (i,j) = FIRST_RISE M (RESTN p i) c (j-i))``,
+   RW_TAC std_ss []
+    THEN `i + (j-i) = j` by DECIDE_TAC
+    THEN PROVE_TAC [FIRST_RISE_RESTN]);
+
 (******************************************************************************
 * Structural induction rule for FL formulas
 ******************************************************************************)
@@ -468,6 +513,15 @@ val PL0 =
    Cases
     THEN RW_TAC std_ss [PL_def,FINITE_PATH_NONEMPTY]);
    
+val FORALL_NOT_PL =
+ store_thm
+  ("FORALL_NOT_PL",
+   ``~!n. ~PL p n``,
+   Cases_on `p`
+    THEN ZAP_TAC arith_ss 
+          [IS_INFINITE_PATH_def,IS_FINITE_PATH_def,
+           PL_def,FINITE_PATH_NONEMPTY]);
+
 val NEXT_TRUE_GE =
  store_thm
   ("NEXT_TRUE_GE",
@@ -488,7 +542,7 @@ val PL_EXISTS_FORALL_LEMMA =
      intLib.COOPER_PROVE``x < n /\ (!x'. x' < n ==> ~(x' >= x)) = F``]);
 
 (******************************************************************************
-* Strong clocking with T equal to weaking clocking with T:
+* Strong clocking with T equal to weak clocking with T:
 * (p |=T!= f  <==>  p |=T= f)
 ******************************************************************************)
 local
@@ -1037,12 +1091,293 @@ val S_CLOCK_COMP_ELIM =
        THEN RW_TAC list_ss [EL_APPEND2]]);
 
 (******************************************************************************
+* Definition of falsity
+******************************************************************************)
+
+val B_FALSE =
+ prove
+  (``B_SEM M l (B_NOT B_TRUE) = F``,
+   RW_TAC std_ss [B_SEM_def]);
+
+(******************************************************************************
 * Some abbreviations needed for definition of F_CLOCK_COMP
 ******************************************************************************)
 
 val F_U_CLOCK_def =
  Define
   `F_U_CLOCK c f = F_UNTIL(F_BOOL(B_NOT c),F_AND(F_BOOL c, f))`;
+
+val UF_SEM_F_U_CLOCK =
+ store_thm
+  ("UF_SEM_F_U_CLOCK",
+   ``UF_SEM M p (F_U_CLOCK c f) =
+      ?i :: PL p. FIRST_RISE M p c i /\ UF_SEM M (RESTN p i) f``,
+   Cases_on `p`
+    THEN RW_TAC arith_ss 
+          [F_U_CLOCK_def,PATH_EL_RESTN,L_def,
+           UF_SEM,B_SEM_def,FIRST_RISE,IS_FINITE_PATH_def,
+           RES_FORALL,RES_EXISTS,PL_def,IN_DEF,NOT_IS_INFINITE_PATH]
+    THEN EQ_TAC
+    THEN RW_TAC std_ss []
+    THEN Q.EXISTS_TAC `x`
+    THEN RW_TAC std_ss []
+    THEN`j < PATH_LENGTH (FINITE_PATH p')` by DECIDE_TAC
+    THEN PROVE_TAC[]);
+
+(******************************************************************************
+* UF_SEM M p (F_U_CLOCK c (F_U_CLOCK c f)) = UF_SEM M p (F_U_CLOCK c f)
+******************************************************************************)
+local
+
+val INFINITE_UF_U_CLOCK_UF_U_CLOCK =
+ prove
+  (``~(IS_FINITE_PATH p)
+     ==>
+     (UF_SEM M p (F_U_CLOCK c (F_U_CLOCK c f)) = UF_SEM M p (F_U_CLOCK c f))``,
+   RW_TAC arith_ss 
+    [F_U_CLOCK_def, UF_SEM,RES_FORALL,RES_EXISTS,PL_def,IN_DEF,
+     PATH_EL_RESTN,RESTN_RESTN,IS_FINITE_PATH_RESTN]
+    THEN EQ_TAC
+    THEN RW_TAC std_ss []
+    THENL
+     [Q.EXISTS_TAC `x+x'`
+       THEN RW_TAC arith_ss []
+       THEN Cases_on `x'' < x`
+       THEN RW_TAC arith_ss []
+       THEN `x'' - x < x'` by DECIDE_TAC
+       THEN `x + (x'' - x) = x''` by DECIDE_TAC
+       THEN PROVE_TAC[],
+      Q.EXISTS_TAC `x`
+       THEN RW_TAC arith_ss []
+       THEN Q.EXISTS_TAC `0`
+       THEN RW_TAC arith_ss [ADD_CLAUSES]]);
+
+val FINITE_UF_U_CLOCK_UF_U_CLOCK =
+ prove
+  (``IS_FINITE_PATH p
+     ==>
+     (UF_SEM M p (F_U_CLOCK c (F_U_CLOCK c f)) = UF_SEM M p (F_U_CLOCK c f))``,
+   RW_TAC arith_ss 
+    [F_U_CLOCK_def, UF_SEM,RES_FORALL,RES_EXISTS,PL_def,IN_DEF,
+     PATH_EL_RESTN,RESTN_RESTN,IS_FINITE_PATH_RESTN]
+    THEN EQ_TAC
+    THEN RW_TAC std_ss []
+    THENL
+     [`PATH_LENGTH(RESTN p x) = PATH_LENGTH p - x` by PROVE_TAC[PATH_LENGTH_RESTN]
+       THEN `x + x' < PATH_LENGTH p` by DECIDE_TAC
+       THEN Q.EXISTS_TAC `x+x'`
+       THEN RW_TAC arith_ss []
+       THEN Cases_on `x'' < x`
+       THEN RW_TAC arith_ss []
+       THEN `x'' - x < x'` by DECIDE_TAC
+       THEN `x + (x'' - x) = x''` by DECIDE_TAC
+       THEN `x'' - x < PATH_LENGTH (RESTN p x)` by DECIDE_TAC
+       THEN PROVE_TAC[],
+      Q.EXISTS_TAC `x`
+       THEN RW_TAC arith_ss []
+       THEN Q.EXISTS_TAC `0`
+       THEN RW_TAC arith_ss [FINITE_PATH_NONEMPTY,ADD_CLAUSES,PATH_LENGTH_RESTN]]);
+in
+
+val UF_U_CLOCK_UF_U_CLOCK =
+ prove
+  (``UF_SEM M p (F_U_CLOCK c (F_U_CLOCK c f)) = UF_SEM M p (F_U_CLOCK c f)``,
+   Cases_on `IS_FINITE_PATH p`
+    THEN RW_TAC std_ss [INFINITE_UF_U_CLOCK_UF_U_CLOCK,FINITE_UF_U_CLOCK_UF_U_CLOCK]);
+
+end;
+
+val F_CLOCK_FREE_F_U_CLOCK  =
+ store_thm
+  ("F_CLOCK_FREE_F_U_CLOCK",
+   ``!f. F_CLOCK_FREE f ==> !c. F_CLOCK_FREE(F_U_CLOCK c f)``,
+   RW_TAC std_ss [F_U_CLOCK_def,F_CLOCK_FREE_def]);
+
+(******************************************************************************
+* F_U_CLOCK_INIT_LEMMA =
+*     |- !i j::PL p.
+*          FIRST_RISE M p c i /\ j <= i ==>
+*          (UF_SEM M (RESTN p j) (F_U_CLOCK c f) = UF_SEM M p (F_U_CLOCK c f))
+******************************************************************************)
+local
+
+val F_U_CLOCK_INFINITE_INIT_LEMMA =
+ prove
+  (``~(IS_FINITE_PATH p)
+     ==>
+     !i i1 :: PL p.
+      FIRST_RISE M p c i /\ i1 <= i
+      ==>
+      (UF_SEM M (RESTN p i1) (F_U_CLOCK c f) = UF_SEM M p (F_U_CLOCK c f))``,
+   RW_TAC arith_ss 
+    [FIRST_RISE,F_U_CLOCK_def,UF_SEM,RES_FORALL,RES_EXISTS,B_SEM_def,
+     RESTN_RESTN,PATH_EL_RESTN,L_def,IN_DEF,PL_def,IS_FINITE_PATH_RESTN]
+    THEN EQ_TAC
+    THEN RW_TAC std_ss []
+    THENL
+     [Q.EXISTS_TAC `x' + x''`
+       THEN RW_TAC arith_ss []
+       THEN Cases_on `x''' < x`
+       THEN RW_TAC arith_ss []
+       THEN IMP_RES_TAC(DECIDE``x' <= x ==> x''' < x' + x'' ==> ~(x''' < x) ==> x''' - x' < x''``)
+       THEN IMP_RES_TAC(DECIDE``x' <= x ==> x''' < x' + x'' ==> ~(x''' < x) ==> (x' + (x''' - x') = x''')``)
+       THEN PROVE_TAC[],
+      Q.EXISTS_TAC `x'' - x'`
+       THEN Cases_on `x'' < x`
+       THEN RES_TAC
+       THEN RW_TAC arith_ss [DECIDE``x' <= x ==> ~(x'' < x) ==> (x' + (x'' - x') = x'')``]]);
+
+val F_U_CLOCK_FINITE_INIT_LEMMA =
+ prove
+  (``IS_FINITE_PATH p
+     ==>
+     !i i1 :: PL p.
+      FIRST_RISE M p c i /\ i1 <= i
+      ==>
+      (UF_SEM M (RESTN p i1) (F_U_CLOCK c f) = UF_SEM M p (F_U_CLOCK c f))``,
+   RW_TAC arith_ss 
+    [FIRST_RISE,F_U_CLOCK_def,UF_SEM,RES_FORALL,RES_EXISTS,B_SEM_def,
+     RESTN_RESTN,PATH_EL_RESTN,L_def,IN_DEF,PL_def,IS_FINITE_PATH_RESTN]
+    THEN EQ_TAC
+    THEN RW_TAC std_ss []
+    THENL
+     [Q.EXISTS_TAC `x' + x''`
+       THEN RW_TAC arith_ss []
+       THEN `PATH_LENGTH (RESTN p x') = PATH_LENGTH p - x'` by RW_TAC arith_ss [PATH_LENGTH_RESTN]
+       THENL
+        [DECIDE_TAC,
+         Cases_on `x''' < x`
+          THEN RW_TAC arith_ss []
+          THEN `x''' - x' < PATH_LENGTH (RESTN p x')` by DECIDE_TAC
+          THEN `x''' - x' < x''` by DECIDE_TAC
+          THEN `x' + (x''' - x') = x'''` by DECIDE_TAC
+          THEN PROVE_TAC[]],
+      Q.EXISTS_TAC `x'' - x'`
+       THEN Cases_on `x'' < x`
+       THEN RES_TAC
+       THEN `PATH_LENGTH (RESTN p x') = PATH_LENGTH p - x'` by RW_TAC arith_ss [PATH_LENGTH_RESTN]
+       THEN `x' + (x'' - x') = x''` by DECIDE_TAC
+       THEN `x'' - x' < PATH_LENGTH p - x'` by DECIDE_TAC
+       THEN RW_TAC std_ss []
+       THEN `x' + x''' < PATH_LENGTH p` by DECIDE_TAC
+       THEN `x' + x''' < x''` by DECIDE_TAC
+       THEN PROVE_TAC[]]);
+
+in
+
+val F_U_CLOCK_INIT_LEMMA =
+ store_thm
+  ("F_U_CLOCK_INIT_LEMMA",
+   ``!i j :: PL p.
+      FIRST_RISE M p c i /\ j <= i
+      ==>
+      (UF_SEM M (RESTN p j) (F_U_CLOCK c f) = UF_SEM M p (F_U_CLOCK c f))``,
+   Cases_on `IS_FINITE_PATH p`
+    THEN RW_TAC std_ss [F_U_CLOCK_INFINITE_INIT_LEMMA,F_U_CLOCK_FINITE_INIT_LEMMA]);
+
+end;
+
+(******************************************************************************
+* F_U_CLOCK_NEXT_LEMMA =
+*     |- !i j k::PL p.
+*          NEXT_RISE M p c (i,j) /\ i <= k /\ k <= j ==>
+*          (UF_SEM M (RESTN p k) (F_U_CLOCK c f) =
+*           UF_SEM M (RESTN p j) (F_U_CLOCK c f)) : thm
+******************************************************************************)
+local
+
+val F_U_CLOCK_INFINITE_NEXT_LEMMA =
+ prove
+  (``~(IS_FINITE_PATH p)
+     ==>
+     !i j k :: PL p.
+      NEXT_RISE M p c (i,j) /\ i <= k /\ k <= j
+      ==>
+      (UF_SEM M (RESTN p k) (F_U_CLOCK c f) = UF_SEM M (RESTN p j) (F_U_CLOCK c f))``,
+   ONCE_REWRITE_TAC[PROVE
+                     [DECIDE``i <= k /\ k <= j==> i <= j``]
+                     ``P /\ i <= k /\ k <= j = ((i <= j) /\ P) /\ i <= k /\ k <= j``]
+    THEN RW_TAC arith_ss 
+        [NEXT_RISE_LESS,F_U_CLOCK_def,UF_SEM,RES_FORALL,RES_EXISTS,B_SEM_def,
+         RESTN_RESTN,PATH_EL_RESTN,L_def,IN_DEF,PL_def,IS_FINITE_PATH_RESTN]
+    THEN EQ_TAC
+    THEN RW_TAC std_ss []
+    THENL
+     [Cases_on `x <= x'' + x''' /\ x'' + x''' < x'`
+       THEN ZAP_TAC arith_ss []
+       THEN `x' + (x'' + x''' - x') = x'' + x''' ` by DECIDE_TAC
+       THEN Q.EXISTS_TAC `x'' + x''' - x'`
+       THEN RW_TAC arith_ss []
+       THEN `x' + x'''' - x'' < x'''` by DECIDE_TAC
+       THEN `x'' + (x' + x'''' - x'') = x' + x''''` by DECIDE_TAC
+       THEN PROVE_TAC[],
+      Q.EXISTS_TAC `x' + x''' - x''`
+       THEN ZAP_TAC std_ss []
+       THEN `x'' + (x' + x''' - x'') = x' + x'''` by DECIDE_TAC
+       THEN ZAP_TAC std_ss []
+       THEN Cases_on `(x <= x'' + x'''' /\ x'' + x'''' < x')`
+       THEN RW_TAC arith_ss []
+       THEN `x'' + x'''' - x' < x'''` by DECIDE_TAC
+       THEN `x' + (x'' + x'''' - x') = x'' + x''''` by DECIDE_TAC
+       THEN PROVE_TAC[]]);
+
+val F_U_CLOCK_FINITE_NEXT_LEMMA =
+ prove
+  (``IS_FINITE_PATH p
+     ==>
+     !i j k :: PL p.
+      NEXT_RISE M p c (i,j) /\ i <= k /\ k <= j
+      ==>
+      (UF_SEM M (RESTN p k) (F_U_CLOCK c f) = UF_SEM M (RESTN p j) (F_U_CLOCK c f))``,
+   ONCE_REWRITE_TAC[PROVE
+                     [DECIDE``i <= k /\ k <= j==> i <= j``]
+                     ``P /\ i <= k /\ k <= j = ((i <= j) /\ P) /\ i <= k /\ k <= j``]
+    THEN RW_TAC arith_ss 
+        [NEXT_RISE_LESS,F_U_CLOCK_def,UF_SEM,RES_FORALL,RES_EXISTS,B_SEM_def,
+         RESTN_RESTN,PATH_EL_RESTN,L_def,IN_DEF,PL_def,IS_FINITE_PATH_RESTN]
+    THEN EQ_TAC
+    THEN RW_TAC std_ss []
+    THENL
+     [Cases_on `x <= x'' + x''' /\ x'' + x''' < x'`
+       THEN ZAP_TAC arith_ss []
+       THEN RW_TAC arith_ss [PATH_LENGTH_RESTN]
+       THEN `x' + (x'' + x''' - x') = x'' + x''' ` by DECIDE_TAC
+       THEN `PATH_LENGTH (RESTN p x'') = PATH_LENGTH p - x''` 
+            by PROVE_TAC[PATH_LENGTH_RESTN]
+       THEN `x'' + x''' < PATH_LENGTH p` by DECIDE_TAC
+       THEN Q.EXISTS_TAC `x'' + x''' - x'`
+       THEN RW_TAC arith_ss []
+       THEN `x' + x''''' - x'' < PATH_LENGTH (RESTN p x'')` by DECIDE_TAC
+       THEN `x' + x''''' - x'' < x'''` by DECIDE_TAC
+       THEN `x'' + (x' + x''''' - x'') = x' + x'''''` by DECIDE_TAC
+       THEN PROVE_TAC[],
+      `PATH_LENGTH (RESTN p x'') = PATH_LENGTH p - x''` 
+        by PROVE_TAC[PATH_LENGTH_RESTN]
+       THEN `PATH_LENGTH (RESTN p x') = PATH_LENGTH p - x'` 
+            by PROVE_TAC[PATH_LENGTH_RESTN]
+       THEN `x'' + (x' + x''' - x'') = x' + x'''` by DECIDE_TAC
+       THEN Q.EXISTS_TAC `x' + x''' - x''`
+       THEN ZAP_TAC std_ss []
+       THEN Cases_on `(x <= x'' + x'''' /\ x'' + x'''' < x')`
+       THEN RW_TAC arith_ss []
+       THEN `x'' + x'''' - x' < PATH_LENGTH (RESTN p x')` by DECIDE_TAC
+       THEN `x'' + x'''' - x' < x'''` by DECIDE_TAC
+       THEN `x' + (x'' + x'''' - x') = x'' + x''''` by DECIDE_TAC
+       THEN PROVE_TAC[]]);
+
+in
+
+val F_U_CLOCK_NEXT_LEMMA =
+ store_thm
+  ("F_U_CLOCK_NEXT_LEMMA",
+   ``!i j k :: PL p.
+      NEXT_RISE M p c (i,j) /\ i <= k /\ k <= j
+      ==>
+      (UF_SEM M (RESTN p k) (F_U_CLOCK c f) = UF_SEM M (RESTN p j) (F_U_CLOCK c f))``,
+   Cases_on `IS_FINITE_PATH p`
+    THEN RW_TAC std_ss [F_U_CLOCK_INFINITE_NEXT_LEMMA,F_U_CLOCK_FINITE_NEXT_LEMMA]);
+
+end;
 
 val F_OR_def =
  Define
@@ -1073,6 +1408,22 @@ val UF_SEM_F_G =
   ("UF_SEM_F_G",
    ``UF_SEM M p (F_G f) = !i :: PL p. UF_SEM M (RESTN p i) f``,
    RW_TAC std_ss [UF_SEM,F_G_def,UF_SEM_F_F,RES_EXISTS,RES_FORALL]
+    THEN PROVE_TAC[]);
+
+val UF_SEM_F_F_G =
+ store_thm
+  ("UF_SEM_F_F_G",
+   ``UF_SEM M p (F_F(F_G f)) = 
+     ?i :: PL p. !j :: PL(RESTN p i). UF_SEM M (RESTN p (i+j)) f``,
+   RW_TAC std_ss [UF_SEM,F_G_def,UF_SEM_F_F,RES_EXISTS,RES_FORALL,RESTN_RESTN]
+    THEN PROVE_TAC[]);
+
+val UF_SEM_F_G_F =
+ store_thm
+  ("UF_SEM_F_G_F",
+   ``UF_SEM M p (F_G(F_F f)) = 
+     !i :: PL p. ?j :: PL(RESTN p i). UF_SEM M (RESTN p (i+j)) f``,
+   RW_TAC std_ss [UF_SEM,F_G_def,UF_SEM_F_F,RES_EXISTS,RES_FORALL,RESTN_RESTN]
     THEN PROVE_TAC[]);
 
 val UF_SEM_NOT_F_G =
@@ -1121,6 +1472,216 @@ val F_W_CLOCK_def =
  Define
   `F_W_CLOCK c f = F_W(F_BOOL(B_NOT c),F_AND(F_BOOL c, f))`;
 
+val UF_SEM_F_W_CLOCK =
+ store_thm
+  ("UF_SEM_F_W_CLOCK",
+   ``UF_SEM M p (F_W_CLOCK c f) = 
+      UF_SEM M p (F_U_CLOCK c f) \/ !i::PL p.~UF_SEM M (RESTN p i) (F_BOOL c)``,
+   RW_TAC std_ss 
+    [F_U_CLOCK_def, F_W_CLOCK_def, UF_SEM_F_W, UF_SEM_F_G,B_SEM_def,UF_SEM_def]);
+
+
+(******************************************************************************
+* F_W_CLOCK_NEXT_LEMMA =
+*     |- !i j k::PL p.
+*          NEXT_RISE M p c (i,j) /\ i <= k /\ k <= j ==>
+*          (UF_SEM M (RESTN p k) (F_W_CLOCK c f) =
+*           UF_SEM M (RESTN p j) (F_W_CLOCK c f)) : thm
+******************************************************************************)
+local
+
+val INFINITE_F_W_CLOCK_NEXT_LEMMA =
+ prove
+  (``~(IS_FINITE_PATH p)
+     ==>
+     !i j k :: PL p.
+      NEXT_RISE M p c (i,j) /\ i <= k /\ k <= j
+      ==>
+      (UF_SEM M (RESTN p k) (F_W_CLOCK c f) = UF_SEM M (RESTN p j) (F_W_CLOCK c f))``,
+    RW_TAC std_ss [UF_SEM_F_W_CLOCK,RES_FORALL,PL_def,IN_DEF,RESTN_RESTN,
+                   IS_FINITE_PATH_RESTN,L_def]
+     THEN EQ_TAC
+     THEN RW_TAC std_ss []
+     THENL
+      [`UF_SEM M (RESTN p x') (F_U_CLOCK c f)`
+        by PROVE_TAC[SIMP_RULE std_ss [RES_FORALL,PL_def,IN_DEF]F_U_CLOCK_NEXT_LEMMA]
+        THEN PROVE_TAC[],
+       DISJ2_TAC
+        THEN RW_TAC std_ss []
+        THEN POP_ASSUM(ASSUME_TAC o Q.SPEC `x' + x''' - x''`)
+        THEN `x'' + (x' + x''' - x'') = x' + x'''` by DECIDE_TAC
+        THEN PROVE_TAC[],
+       `UF_SEM M (RESTN p x'') (F_U_CLOCK c f)`
+        by PROVE_TAC[SIMP_RULE std_ss [RES_FORALL,PL_def,IN_DEF]F_U_CLOCK_NEXT_LEMMA]
+        THEN PROVE_TAC[],
+       DISJ2_TAC
+        THEN RW_TAC arith_ss []
+        THEN FULL_SIMP_TAC arith_ss [UF_SEM,PATH_EL_RESTN]
+        THEN `x <= x'` by DECIDE_TAC
+        THEN ASSUM_LIST
+              (fn thl => 
+                STRIP_ASSUME_TAC
+                 (SIMP_RULE std_ss [NEXT_RISE_LESS] (CONJ(el 1 thl)(el 5 thl))))
+        THEN `x <= x'' + x'''` by DECIDE_TAC
+        THEN Cases_on `x'' + x''' < x'`
+        THEN RW_TAC arith_ss [L_def]
+        THEN FULL_SIMP_TAC std_ss [L_def]
+        THEN `x'' + x''' = x' + (x'' + x''' - x')` by DECIDE_TAC
+        THEN ASSUM_LIST(fn thl => ASSUME_TAC(SPEC ``x'' + x''' - x'`` (el 7 thl)))
+        THEN PROVE_TAC[]]);
+
+val FINITE_F_W_CLOCK_NEXT_LEMMA =
+ prove
+  (``IS_FINITE_PATH p
+     ==>
+     !i j k :: PL p.
+      NEXT_RISE M p c (i,j) /\ i <= k /\ k <= j
+      ==>
+      (UF_SEM M (RESTN p k) (F_W_CLOCK c f) = UF_SEM M (RESTN p j) (F_W_CLOCK c f))``,
+    RW_TAC std_ss [UF_SEM_F_W_CLOCK,RES_FORALL,PL_def,IN_DEF,RESTN_RESTN,
+                   IS_FINITE_PATH_RESTN,L_def]
+     THEN EQ_TAC
+     THEN RW_TAC std_ss []
+     THENL
+      [`UF_SEM M (RESTN p x') (F_U_CLOCK c f)`
+        by PROVE_TAC[SIMP_RULE std_ss [RES_FORALL,PL_def,IN_DEF]F_U_CLOCK_NEXT_LEMMA]
+        THEN PROVE_TAC[],
+       DISJ2_TAC
+        THEN RW_TAC std_ss []
+        THEN ASSUM_LIST(fn thl => ASSUME_TAC(Q.SPEC `x' + x''' - x''` (el 2 thl)))
+        THEN `x'' + (x' + x''' - x'') = x' + x'''` by DECIDE_TAC
+        THEN `PATH_LENGTH (RESTN p x'') = PATH_LENGTH p - x''` by PROVE_TAC[PATH_LENGTH_RESTN]
+        THEN `PATH_LENGTH (RESTN p x') = PATH_LENGTH p - x'` by PROVE_TAC[PATH_LENGTH_RESTN]
+        THEN `x' + x''' - x'' < PATH_LENGTH (RESTN p x'')` by DECIDE_TAC
+        THEN PROVE_TAC[],
+       `UF_SEM M (RESTN p x'') (F_U_CLOCK c f)`
+        by PROVE_TAC[SIMP_RULE std_ss [RES_FORALL,PL_def,IN_DEF]F_U_CLOCK_NEXT_LEMMA]
+        THEN PROVE_TAC[],
+       DISJ2_TAC
+        THEN RW_TAC arith_ss []
+        THEN FULL_SIMP_TAC arith_ss [UF_SEM,PATH_EL_RESTN]
+        THEN `x <= x'` by DECIDE_TAC
+        THEN ASSUM_LIST
+              (fn thl => 
+                STRIP_ASSUME_TAC
+                 (SIMP_RULE std_ss [NEXT_RISE_LESS] (CONJ(el 1 thl)(el 6 thl))))
+        THEN `x <= x'' + x'''` by DECIDE_TAC
+        THEN Cases_on `x'' + x''' < x'`
+        THEN RW_TAC arith_ss [L_def]
+        THEN FULL_SIMP_TAC std_ss [L_def]
+        THEN `x'' + x''' = x' + (x'' + x''' - x')` by DECIDE_TAC
+        THEN ASSUM_LIST(fn thl => ASSUME_TAC(SPEC ``x'' + x''' - x'`` (el 8 thl)))
+        THEN `PATH_LENGTH (RESTN p x') = PATH_LENGTH p - x'` by PROVE_TAC[PATH_LENGTH_RESTN]
+        THEN `PATH_LENGTH (RESTN p x'') = PATH_LENGTH p - x''` by PROVE_TAC[PATH_LENGTH_RESTN]
+        THEN `x'' + x''' - x' < PATH_LENGTH (RESTN p x')` by DECIDE_TAC
+        THEN PROVE_TAC[]]);
+
+in
+
+val F_W_CLOCK_NEXT_LEMMA =
+ store_thm
+  ("F_W_CLOCK_NEXT_LEMMA",
+   ``!i j k :: PL p.
+      NEXT_RISE M p c (i,j) /\ i <= k /\ k <= j
+      ==>
+      (UF_SEM M (RESTN p k) (F_W_CLOCK c f) = UF_SEM M (RESTN p j) (F_W_CLOCK c f))``,
+   Cases_on `IS_FINITE_PATH p`
+    THEN RW_TAC std_ss [INFINITE_F_W_CLOCK_NEXT_LEMMA,FINITE_F_W_CLOCK_NEXT_LEMMA]);
+
+end;
+
+(******************************************************************************
+* UF_W_CLOCK_UF_W_CLOCK =
+*  |- UF_SEM M p (F_W_CLOCK c (F_W_CLOCK c f)) = UF_SEM M p (F_W_CLOCK c f) 
+******************************************************************************)
+local
+
+val INFINITE_UF_W_CLOCK_UF_W_CLOCK =
+ prove
+  (``~(IS_FINITE_PATH p)
+     ==>
+     (UF_SEM M p (F_W_CLOCK c (F_W_CLOCK c f)) = UF_SEM M p (F_W_CLOCK c f))``,
+    RW_TAC std_ss [UF_SEM_F_W_CLOCK,RES_FORALL,PL_def,IN_DEF,RESTN_RESTN,
+                   IS_FINITE_PATH_RESTN,L_def,UF_U_CLOCK_UF_U_CLOCK]
+     THEN EQ_TAC
+     THEN RW_TAC arith_ss 
+           [F_W_CLOCK_def,F_U_CLOCK_def,F_OR_def,F_F_def,RESTN_RESTN,
+            F_G_def,F_W_def,F_W_CLOCK_def,UF_SEM,PATH_EL_RESTN,B_SEM_def,
+            RES_FORALL,RES_EXISTS,PL_def,IN_DEF,L_def,IS_FINITE_PATH_RESTN]
+     THEN RW_TAC std_ss []
+     THENL
+      [DISJ1_TAC
+        THEN Q.EXISTS_TAC`x+x'`
+        THEN RW_TAC std_ss []
+        THEN Cases_on `x'' < x`
+        THEN RW_TAC std_ss []
+        THEN FULL_SIMP_TAC std_ss [DECIDE ``~(m < n) \/ P = m < n ==> P``]
+        THEN `(x'' - x) < x'` by DECIDE_TAC
+        THEN `x + (x'' - x) = x''` by DECIDE_TAC
+        THEN PROVE_TAC[],
+       ASSUM_LIST(fn thl => ASSUME_TAC(SIMP_RULE arith_ss [] (SPEC ``0`` (el 2 thl))))
+        THEN PROVE_TAC[],
+       DISJ1_TAC
+        THEN Q.EXISTS_TAC`x`
+        THEN RW_TAC std_ss []
+        THEN DISJ1_TAC
+        THEN Q.EXISTS_TAC `0`
+        THEN RW_TAC arith_ss []]);
+      
+
+val FINITE_UF_W_CLOCK_UF_W_CLOCK =
+ prove
+  (``IS_FINITE_PATH p
+     ==>
+     (UF_SEM M p (F_W_CLOCK c (F_W_CLOCK c f)) = UF_SEM M p (F_W_CLOCK c f))``,
+    RW_TAC std_ss [UF_SEM_F_W_CLOCK,RES_FORALL,PL_def,IN_DEF,RESTN_RESTN,
+                   IS_FINITE_PATH_RESTN,L_def,UF_U_CLOCK_UF_U_CLOCK]
+     THEN EQ_TAC
+     THEN RW_TAC arith_ss 
+           [F_W_CLOCK_def,F_U_CLOCK_def,F_OR_def,F_F_def,RESTN_RESTN,
+            F_G_def,F_W_def,F_W_CLOCK_def,UF_SEM,PATH_EL_RESTN,B_SEM_def,
+            RES_FORALL,RES_EXISTS,PL_def,IN_DEF,L_def,IS_FINITE_PATH_RESTN]
+     THEN RW_TAC std_ss []
+     THENL
+      [DISJ1_TAC
+        THEN Q.EXISTS_TAC`x+x'`
+        THEN RW_TAC std_ss []
+        THEN `PATH_LENGTH (RESTN p x) = PATH_LENGTH p - x` by PROVE_TAC[PATH_LENGTH_RESTN]
+        THEN `x + x' < PATH_LENGTH p` by DECIDE_TAC
+        THEN RW_TAC std_ss []
+        THEN FULL_SIMP_TAC std_ss [DECIDE ``~(m < n) \/ P = m < n ==> P``]
+        THEN Cases_on `x'' < x`
+        THEN RW_TAC std_ss []
+        THEN `(x'' - x) < x'` by DECIDE_TAC
+        THEN `(x'' - x) < PATH_LENGTH p - x` by DECIDE_TAC
+        THEN `x + (x'' - x) = x''` by DECIDE_TAC
+        THEN PROVE_TAC[],
+       ASSUM_LIST(fn thl => ASSUME_TAC(SIMP_RULE arith_ss [] (SPEC ``0`` (el 2 thl))))
+        THEN PROVE_TAC[FINITE_PATH_NONEMPTY,IS_FINITE_PATH_RESTN],
+       DISJ1_TAC
+        THEN Q.EXISTS_TAC`x`
+        THEN RW_TAC std_ss []
+        THEN DISJ1_TAC
+        THEN Q.EXISTS_TAC `0`
+        THEN RW_TAC arith_ss [FINITE_PATH_NONEMPTY,IS_FINITE_PATH_RESTN]]);
+      
+in
+
+val UF_W_CLOCK_UF_W_CLOCK =
+ store_thm
+  ("UF_W_CLOCK_UF_W_CLOCK",
+   ``UF_SEM M p (F_W_CLOCK c (F_W_CLOCK c f)) = UF_SEM M p (F_W_CLOCK c f)``,
+   Cases_on `IS_FINITE_PATH p`
+    THEN RW_TAC std_ss [INFINITE_UF_W_CLOCK_UF_W_CLOCK,FINITE_UF_W_CLOCK_UF_W_CLOCK]);
+
+end;
+
+val F_CLOCK_FREE_F_W_CLOCK  =
+ store_thm
+  ("F_CLOCK_FREE_F_W_CLOCK",
+   ``!f. F_CLOCK_FREE f ==> !c. F_CLOCK_FREE(F_W_CLOCK c f)``,
+   RW_TAC std_ss [F_W_CLOCK_def,F_G_def,F_F_def,F_W_def,F_OR_def,F_CLOCK_FREE_def]);
+
 (******************************************************************************
 * Rules for compiling clocked FL formulas to unclocked formulas
 * (from B.1, page 66 and 67, of Sugar 2.0 Accellera document)
@@ -1152,6 +1713,7 @@ val F_CLOCK_COMP_def =
       F_U_CLOCK c (F_STRONG_IMP (S_CLOCK_COMP c r1,
                                  S_CLOCK_COMP c r2)))
     /\
+
     (F_CLOCK_COMP (STRONG_CLOCK c) (F_WEAK_IMP(r1,r2)) = 
       F_U_CLOCK c (F_OR
                     (F_STRONG_IMP(S_CLOCK_COMP c r1, S_CLOCK_COMP c r2),
@@ -1235,18 +1797,154 @@ val F_CLOCK_COMP_CLOCK_FREE =
    Cases
     THEN RW_TAC std_ss [F_CLOCK_COMP_CLOCK_FREE_LEMMA]);
 
+val F_U_CLOCK_F_U_CLOCK =
+ prove
+  (``F_SEM M p (STRONG_CLOCK B_TRUE) 
+               (F_U_CLOCK c (F_U_CLOCK c (F_CLOCK_COMP (STRONG_CLOCK B_TRUE) f))) = 
+      F_SEM M p (STRONG_CLOCK B_TRUE) 
+                (F_U_CLOCK c (F_CLOCK_COMP (STRONG_CLOCK B_TRUE) f))``,
+   PROVE_TAC
+    [F_SEM_STRONG_FREE_TRUE_LEMMA,UF_U_CLOCK_UF_U_CLOCK, 
+     F_CLOCK_COMP_CLOCK_FREE_LEMMA,F_CLOCK_FREE_F_U_CLOCK]);
+
+val F_W_CLOCK_F_W_CLOCK =
+ prove
+  (``F_SEM M p (STRONG_CLOCK B_TRUE) 
+               (F_W_CLOCK c (F_W_CLOCK c (F_CLOCK_COMP (STRONG_CLOCK B_TRUE) f))) = 
+      F_SEM M p (STRONG_CLOCK B_TRUE) 
+                (F_W_CLOCK c (F_CLOCK_COMP (STRONG_CLOCK B_TRUE) f))``,
+   PROVE_TAC
+    [F_SEM_STRONG_FREE_TRUE_LEMMA,UF_W_CLOCK_UF_W_CLOCK, 
+     F_CLOCK_COMP_CLOCK_FREE_LEMMA,F_CLOCK_FREE_F_W_CLOCK]);
+
 (******************************************************************************
-* CLOCK_COMP_HYP f  =  (p |=k= f  <==>  p |= (F_CLOCK_COMP k f))
+* Key property of formulas that only evaluate on clock edges
+******************************************************************************)
+
+val CLOCK_COMP_STABLE_def =
+ Define
+  `CLOCK_COMP_STABLE M c f =
+    !p. (UF_SEM M p (F_U_CLOCK c (F_CLOCK_COMP (STRONG_CLOCK c) f)) = 
+          UF_SEM M p (F_CLOCK_COMP (STRONG_CLOCK c) f))
+        /\
+        (UF_SEM M p (F_W_CLOCK c (F_CLOCK_COMP (WEAK_CLOCK c) f)) = 
+          UF_SEM M p (F_CLOCK_COMP (WEAK_CLOCK c) f))`;     
+
+
+val INFINITE_F_U_CLOCK_STABLE_def =
+ Define
+  `INFINITE_F_U_CLOCK_STABLE M c f = 
+    !p. IS_INFINITE_PATH p ==> (UF_SEM M p (F_U_CLOCK c f) = UF_SEM M p f) `;
+
+val INFINITE_F_W_CLOCK_STABLE_def =
+ Define
+  `INFINITE_F_W_CLOCK_STABLE M c f = 
+    !p. IS_INFINITE_PATH p ==> (UF_SEM M p (F_W_CLOCK c f) = UF_SEM M p f) `;
+
+val FINITE_F_U_CLOCK_STABLE_def =
+ Define
+  `FINITE_F_U_CLOCK_STABLE M c f = 
+    !p. IS_FINITE_PATH p ==> (UF_SEM M p (F_U_CLOCK c f) = UF_SEM M p f) `;
+
+val FINITE_F_W_CLOCK_STABLE_def =
+ Define
+  `FINITE_F_W_CLOCK_STABLE M c f = 
+    !p. IS_FINITE_PATH p ==> (UF_SEM M p (F_W_CLOCK c f) = UF_SEM M p f) `;
+
+(******************************************************************************
+* Compiled strong clocking with T equal to compiled weak clocking with T:
+******************************************************************************)
+local
+
+val INIT_TAC =
+ RW_TAC std_ss 
+  [UF_SEM,FIRST_RISE_TRUE,B_SEM_def,RES_FORALL,RES_EXISTS,IN_DEF,PL0,
+   NEXT_RISE_TRUE_EXISTS,RESTN_def,IS_FINITE_PATH_RESTN,RESTN_RESTN,
+   F_CLOCK_COMP_def,F_U_CLOCK_def,F_OR_def,F_F_def,
+   F_G_def,F_W_def,F_W_CLOCK_def,NOT_IS_INFINITE_PATH,
+   RES_FORALL,RES_EXISTS,IN_DEF,FORALL_NOT_PL]
+ THEN TRY(PROVE_TAC[]);
+
+in
+
+val F_SEM_CLOCK_COMP_TRUE_EQ =
+ store_thm
+  ("F_SEM_CLOCK_COMP_TRUE_EQ",
+   ``!f M p. 
+      UF_SEM M p (F_CLOCK_COMP (STRONG_CLOCK B_TRUE) f) = 
+       UF_SEM M p (F_CLOCK_COMP (WEAK_CLOCK B_TRUE) f)``,
+   INDUCT_THEN fl_induct ASSUME_TAC
+    THENL
+     [(* F_BOOL b *)
+      INIT_TAC,
+      (* F_NOT b *)
+      INIT_TAC,
+      (* F_AND (f1,f2) *)
+      INIT_TAC,
+      (* F_NEXT f *)
+      INIT_TAC,
+      (* F_UNTIL(f1,f2) f *)
+      REPEAT GEN_TAC
+       THEN Cases_on `IS_FINITE_PATH p`
+       THEN INIT_TAC
+       THEN RW_TAC arith_ss
+             [PL_def,IN_DEF,PL_EXISTS_FORALL_LEMMA,FINITE_PATH_NONEMPTY,
+              IS_FINITE_PATH_def,IS_FINITE_PATH_RESTN]
+       THEN EQ_TAC
+       THEN RW_TAC std_ss []
+       THEN Q.EXISTS_TAC `x`
+       THEN RW_TAC std_ss []
+       THEN PROVE_TAC[],
+      (* F_SUFFIX_IMP(s,f) *)
+      INIT_TAC
+       THEN EQ_TAC
+       THEN RW_TAC std_ss []
+       THEN Q.EXISTS_TAC `x`
+       THEN RW_TAC std_ss []
+       THEN PROVE_TAC[],
+      (* F_STRONG_IMP(s1,s2) *)
+      INIT_TAC
+       THEN EQ_TAC
+       THEN RW_TAC std_ss []
+       THEN Q.EXISTS_TAC `x`
+       THEN RW_TAC std_ss []
+       THEN PROVE_TAC[],
+      (* F_WEAK_IMP(s1,s2) *)
+      INIT_TAC
+       THEN EQ_TAC
+       THEN RW_TAC std_ss []
+       THEN Q.EXISTS_TAC `x`
+       THEN RW_TAC std_ss []
+       THEN PROVE_TAC[],
+      (* F_ABORT(f,b)) *)
+      INIT_TAC
+       THEN EQ_TAC
+       THEN RW_TAC std_ss []
+       THEN Q.EXISTS_TAC `x`
+       THEN RW_TAC std_ss []
+       THEN PROVE_TAC[],
+      (* F_WEAK_CLOCK(f,c) *)
+      INIT_TAC,
+      (* F_STRONG_CLOCK(f,c) *)
+      INIT_TAC]);
+
+end;
+
+(******************************************************************************
+* CLOCK_COMP_CORRECT f  =  (p |=k= f  <==>  p |= (F_CLOCK_COMP k f))
 * where k is (STRONG_CLOCK c) or (WEAK_CLOCK c)
 *
-* We prove lemmas CLOCK_COMP_HYP M f for various cases of f.
+* We prove lemmas CLOCK_COMP_CORRECT M f for various cases of f.
 * Note that we cannot define 
-*   |- CLOCK_COMP_HYP f = !M. ...
+*   |- CLOCK_COMP_CORRECT f = !M. ...
 * because there would then be unbound types variables in the rhs.
+*
+* Cindy Eisner formulation: pi |=T f <==> pi |=T ClockComp(f) (IMHO wrong)
+*
 ******************************************************************************)
-val CLOCK_COMP_HYP_def =
+val CLOCK_COMP_CORRECT_def =
  Define
-  `CLOCK_COMP_HYP M f =
+  `CLOCK_COMP_CORRECT M f =
     !p c. (F_SEM M p (STRONG_CLOCK c) f =
             UF_SEM M p (F_CLOCK_COMP (STRONG_CLOCK c) f))
           /\
@@ -1259,9 +1957,9 @@ val F_BOOL_STRONG_CLOCK_COMP_ELIM =
    ``!b M p c.
       F_SEM M p (STRONG_CLOCK c) (F_BOOL b) =
        UF_SEM M p (F_CLOCK_COMP (STRONG_CLOCK c) (F_BOOL b))``,
-   RW_TAC std_ss [F_SEM_def, UF_SEM_def, F_CLOCK_COMP_def,PATH_EL_RESTN,
-                  F_U_CLOCK_def, F_W_CLOCK_def,FIRST_RISE,B_SEM_def,L_def,
-                  RES_FORALL,RES_EXISTS,PL_def,pred_setTheory.SPECIFICATION]
+   RW_TAC arith_ss [F_SEM_def, UF_SEM_def, F_CLOCK_COMP_def,PATH_EL_RESTN,
+                    F_U_CLOCK_def, F_W_CLOCK_def,FIRST_RISE,B_SEM_def,L_def,
+                    RES_FORALL,RES_EXISTS,PL_def,pred_setTheory.SPECIFICATION]
     THEN EQ_TAC
     THEN RW_TAC std_ss []
     THENL
@@ -1294,16 +1992,16 @@ val F_BOOL_WEAK_CLOCK_COMP_ELIM =
    ``!b M p c.
       F_SEM M p (WEAK_CLOCK c) (F_BOOL b) =
        UF_SEM M p (F_CLOCK_COMP (WEAK_CLOCK c) (F_BOOL b))``,
-   RW_TAC std_ss [F_SEM_def, UF_SEM_def, F_CLOCK_COMP_def,F_W_CLOCK_def,
-                  UF_SEM_F_W,FIRST_RISE,PATH_EL_RESTN]
+   RW_TAC arith_ss [F_SEM_def, UF_SEM_def, F_CLOCK_COMP_def,F_W_CLOCK_def,
+                    UF_SEM_F_W,FIRST_RISE,PATH_EL_RESTN]
     THEN Cases_on `UF_SEM M p (F_G (F_BOOL (B_NOT c)))`
     THEN RW_TAC std_ss []
     THENL
      [RW_TAC std_ss [RES_FORALL, IN_DEF]
-       THEN FULL_SIMP_TAC std_ss 
+       THEN FULL_SIMP_TAC arith_ss 
              [UF_SEM,B_SEM_def,UF_SEM_F_G,RES_FORALL,IN_DEF,PATH_EL_RESTN,L_def]
        THEN RES_TAC,
-      FULL_SIMP_TAC std_ss 
+      FULL_SIMP_TAC arith_ss 
             [UF_SEM_WOP_NOT_F_G,RES_FORALL,RES_EXISTS,IN_DEF,UF_SEM,
              PATH_EL_RESTN,B_SEM_def,L_def]
        THEN RW_TAC std_ss [RES_FORALL,RES_EXISTS,IN_DEF,B_SEM_def]
@@ -1319,16 +2017,16 @@ val F_BOOL_WEAK_CLOCK_COMP_ELIM =
 val F_BOOL_CLOCK_COMP_ELIM =
  store_thm
   ("F_BOOL_CLOCK_COMP_ELIM",
-   ``!M b. CLOCK_COMP_HYP M (F_BOOL b)``,
+   ``!M b. CLOCK_COMP_CORRECT M (F_BOOL b)``,
    RW_TAC std_ss 
-    [CLOCK_COMP_HYP_def,
+    [CLOCK_COMP_CORRECT_def,
      F_BOOL_WEAK_CLOCK_COMP_ELIM,F_BOOL_STRONG_CLOCK_COMP_ELIM]);
 
 val F_NOT_CLOCK_COMP_ELIM =
  store_thm
   ("F_NOT_CLOCK_COMP_ELIM",
-   ``!M f. CLOCK_COMP_HYP M f ==> CLOCK_COMP_HYP M (F_NOT f)``,
-   RW_TAC std_ss [CLOCK_COMP_HYP_def,F_SEM_def,UF_SEM,F_CLOCK_COMP_def]);
+   ``!M f. CLOCK_COMP_CORRECT M f ==> CLOCK_COMP_CORRECT M (F_NOT f)``,
+   RW_TAC std_ss [CLOCK_COMP_CORRECT_def,F_SEM_def,UF_SEM,F_CLOCK_COMP_def]);
 
 val F_AND_CLOCK_COMP_ELIM_LEMMA =
  prove
@@ -1348,18 +2046,18 @@ val WOP_LESS =
 
 val F_AND_CLOCK_COMP_ELIM =
  store_thm
-  ("F_NOT_CLOCK_COMP_ELIM",
-   ``!M f1 f2. CLOCK_COMP_HYP M f1 /\ CLOCK_COMP_HYP M f2 
-               ==> CLOCK_COMP_HYP M (F_AND(f1,f2))``,
-   RW_TAC std_ss 
-    [CLOCK_COMP_HYP_def,F_SEM_def,UF_SEM,F_CLOCK_COMP_def,
+  ("F_AND_CLOCK_COMP_ELIM",
+   ``!M f1 f2. CLOCK_COMP_CORRECT M f1 /\ CLOCK_COMP_CORRECT M f2 
+               ==> CLOCK_COMP_CORRECT M (F_AND(f1,f2))``,
+   RW_TAC arith_ss 
+    [CLOCK_COMP_CORRECT_def,F_SEM_def,UF_SEM,F_CLOCK_COMP_def,
      FIRST_RISE,F_U_CLOCK_def,F_W_CLOCK_def,F_W_def,F_OR_def,
      PATH_EL_RESTN,RES_FORALL,RES_EXISTS,L_def,B_SEM_def,IN_DEF]
     THEN REWRITE_TAC[DECIDE``~A\/B = A==>B``]
     THEN TRY(PROVE_TAC[PL_LESS_MONO])
     THEN Cases_on `UF_SEM M p (F_G (F_BOOL (B_NOT c)))`
     THEN RW_TAC std_ss []
-    THEN FULL_SIMP_TAC std_ss 
+    THEN FULL_SIMP_TAC arith_ss 
           [UF_SEM_F_G,RES_FORALL,IN_DEF,UF_SEM,L_def,PATH_EL_RESTN,B_SEM_def]
     THEN RES_TAC
     THEN REWRITE_TAC
@@ -1383,19 +2081,1542 @@ val F_AND_CLOCK_COMP_ELIM =
        THEN MAP_EVERY Cases_on [`x''< x`, `x < x''`, `x'< x`, `x < x'`]
        THEN PROVE_TAC[DECIDE``~(m < n)==>~(n < m)==>(m=n)``]]);
 
-
-(* Goal:
-val F_CLOCK_COMP_ELIM =
+val F_SUFFIX_IMP_CLOCK_COMP_ELIM =
  store_thm
-  ("F_CLOCK_COMP_ELIM",
-   ``!f M CLOCK_COMP_HYP M f``
-   INDUCT_THEN fl_induct ASSUME_TAC
-    THEN RW_TAC std_ss [CLOCK_COMP_HYP_def]
+  ("F_SUFFIX_IMP_CLOCK_COMP_ELIM",
+   ``!M r f. CLOCK_COMP_CORRECT M f
+           ==> CLOCK_COMP_CORRECT M (F_SUFFIX_IMP(r,f))``,
+   RW_TAC arith_ss 
+    [CLOCK_COMP_CORRECT_def,F_SEM_def,UF_SEM,F_CLOCK_COMP_def,
+     F_W_CLOCK_def,F_U_CLOCK_def,PATH_EL_RESTN,L_def,
+     UF_SEM_F_W,UF_SEM_F_G,
+     UF_SEM,B_SEM_def,FIRST_RISE,IS_FINITE_PATH_def,
+     RES_FORALL,RES_EXISTS,PL_def,IN_DEF,NOT_IS_INFINITE_PATH]
+    THEN Cases_on `IS_INFINITE_PATH p`
+    THEN FULL_SIMP_TAC std_ss [NOT_IS_INFINITE_PATH]
+    THEN RW_TAC std_ss []
+    THENL
+     [EQ_TAC
+       THEN RW_TAC std_ss []
+       THENL
+        [Q.EXISTS_TAC `x`
+          THEN RW_TAC std_ss [RESTN_RESTN]
+          THEN FULL_SIMP_TAC arith_ss 
+                [GSYM S_CLOCK_COMP_ELIM,PATH_SEG_RESTN],
+         Q.EXISTS_TAC `x`
+          THEN RW_TAC std_ss [RESTN_RESTN]
+          THEN ASSUM_LIST(fn thl => 
+                           FULL_SIMP_TAC arith_ss 
+                            [el 6 thl,IS_FINITE_PATH_RESTN,PATH_SEG_RESTN,
+                             GSYM S_CLOCK_COMP_ELIM,RESTN_RESTN])
+          THEN `x + (x' - x) = x'` by DECIDE_TAC
+          THEN PROVE_TAC[]],
+      EQ_TAC
+       THEN RW_TAC std_ss []
+       THENL
+        [Q.EXISTS_TAC `x`
+          THEN RW_TAC std_ss []
+          THEN ASSUM_LIST(fn thl => 
+                           FULL_SIMP_TAC arith_ss 
+                            [el 6 thl,IS_FINITE_PATH_RESTN,PATH_SEG_RESTN,
+                             GSYM S_CLOCK_COMP_ELIM,RESTN_RESTN]
+                           THEN ASSUME_TAC(el 6 thl))
+          THEN RES_TAC
+          THEN `PATH_LENGTH (RESTN p x) = PATH_LENGTH p - x` by PROVE_TAC[PATH_LENGTH_RESTN]
+          THEN `x + x' < PATH_LENGTH p` by DECIDE_TAC
+          THEN PROVE_TAC[DECIDE``x <= x + x'``],
+         Q.EXISTS_TAC `x`
+          THEN RW_TAC std_ss [RESTN_RESTN]
+          THENL[`j < PATH_LENGTH p` by DECIDE_TAC THEN PROVE_TAC[], ALL_TAC]
+          THEN ASSUM_LIST(fn thl => 
+                           FULL_SIMP_TAC arith_ss 
+                            [el 7 thl,el 8 thl, IS_FINITE_PATH_RESTN,PATH_SEG_RESTN,
+                             GSYM S_CLOCK_COMP_ELIM,RESTN_RESTN]
+                           THEN ASSUME_TAC(el 7 thl) THEN ASSUME_TAC(el 8 thl))
+          THEN `PATH_LENGTH (RESTN p x) = PATH_LENGTH p - x` by PROVE_TAC[PATH_LENGTH_RESTN]
+          THEN `x + (x' - x) = x'` by DECIDE_TAC
+          THEN `x' - x < PATH_LENGTH(RESTN p x)` by DECIDE_TAC
+          THEN PROVE_TAC[]],
+      EQ_TAC
+       THEN RW_TAC std_ss []
+       THENL
+        [Cases_on `!x. ~B_SEM M (getL M (PATH_EL p x)) c`
+          THEN RW_TAC std_ss []
+          THEN FULL_SIMP_TAC std_ss [NOT_FORALL_THM]
+          THEN ASSUM_LIST
+                (fn thl => ASSUME_TAC(SIMP_RULE std_ss [] (Q.ISPEC `\x. ^(concl(el 1 thl))` WOP)))
+          THEN `?n. B_SEM M (getL M (PATH_EL p n)) c /\
+                    !m. m < n ==> ~B_SEM M (getL M (PATH_EL p m)) c`
+               by PROVE_TAC[]
+          THEN Q.EXISTS_TAC `n`
+          THEN RW_TAC std_ss [RESTN_RESTN]
+          THEN FULL_SIMP_TAC arith_ss 
+                [GSYM S_CLOCK_COMP_ELIM,PATH_SEG_RESTN]
+          THEN `!x'. n <= x' /\ S_SEM M (LHAT M (PATH_SEG p (n,x'))) c r ==>
+                     UF_SEM M (RESTN p x') (F_CLOCK_COMP (WEAK_CLOCK c) f)`
+               by PROVE_TAC[]
+          THEN PROVE_TAC[DECIDE``n <= n + x'``],
+         ASSUM_LIST(fn thl => 
+                     FULL_SIMP_TAC arith_ss 
+                      [el 8 thl,IS_FINITE_PATH_RESTN,PATH_SEG_RESTN,
+                       GSYM S_CLOCK_COMP_ELIM,RESTN_RESTN])
+          THEN Cases_on `x < x'`
+          THEN Cases_on `x' < x`
+          THEN RES_TAC
+          THEN `x=x'` by DECIDE_TAC
+          THEN RW_TAC std_ss []
+          THEN PROVE_TAC[DECIDE ``x <= x'' ==> (x + (x'' - x) = x'')``],
+         PROVE_TAC[L_def]],
+      EQ_TAC
+       THEN RW_TAC std_ss []
+       THENL
+        [Cases_on `!x. x < PATH_LENGTH p ==> ~B_SEM M (getL M (PATH_EL p x)) c`
+          THEN RW_TAC std_ss []
+          THEN FULL_SIMP_TAC std_ss [NOT_FORALL_THM]
+          THEN ASSUM_LIST
+                (fn thl => ASSUME_TAC
+                            (SIMP_RULE std_ss [] 
+                              (Q.ISPEC `\x. ^(concl(el 2 thl)) /\ ^(concl(el 1 thl))` WOP)))
+          THEN `?n. n < PATH_LENGTH p /\ B_SEM M (getL M (PATH_EL p n)) c /\
+                    !m. m < PATH_LENGTH p ==> m < n ==> ~B_SEM M (getL M (PATH_EL p m)) c`
+               by PROVE_TAC[]
+          THEN Q.EXISTS_TAC `n`
+          THEN RW_TAC std_ss [RESTN_RESTN]
+          THEN FULL_SIMP_TAC arith_ss 
+                [GSYM S_CLOCK_COMP_ELIM,PATH_SEG_RESTN]
+          THEN `!j. j < n ==> j < PATH_LENGTH p` by DECIDE_TAC
+          THEN `!j. j < n ==> ~B_SEM M (getL M (PATH_EL p j)) c`
+                by PROVE_TAC[]
+          THEN `!x'. x' < PATH_LENGTH p ==>
+                     n <= x' /\ S_SEM M (LHAT M (PATH_SEG p (n,x'))) c r ==>
+                     UF_SEM M (RESTN p x') (F_CLOCK_COMP (WEAK_CLOCK c) f)`
+               by PROVE_TAC[]
+          THEN `PATH_LENGTH (RESTN p n) = PATH_LENGTH p - n` by PROVE_TAC[PATH_LENGTH_RESTN]
+          THEN FULL_SIMP_TAC std_ss [IS_FINITE_PATH_RESTN]
+          THEN `x' < PATH_LENGTH p - n` by PROVE_TAC[]
+          THEN PROVE_TAC
+                [DECIDE``x < PATH_LENGTH p ==> x' < PATH_LENGTH p - n ==> n + x' < PATH_LENGTH p``,
+                 DECIDE ``n <= n + x'``],
+         ASSUM_LIST(fn thl => 
+                     FULL_SIMP_TAC arith_ss 
+                      [el 11 thl,IS_FINITE_PATH_RESTN,PATH_SEG_RESTN,
+                       GSYM S_CLOCK_COMP_ELIM,RESTN_RESTN]
+                     THEN ASSUME_TAC(el 11 thl))
+          THEN `PATH_LENGTH (RESTN p x) = PATH_LENGTH p - x` by PROVE_TAC[PATH_LENGTH_RESTN]
+          THEN `x' < PATH_LENGTH p` by DECIDE_TAC
+          THEN Cases_on `x < x'`
+          THEN Cases_on `x' < x`
+          THEN RES_TAC
+          THEN `x=x'` by DECIDE_TAC
+          THEN RW_TAC std_ss []
+          THEN IMP_RES_TAC(DECIDE``(m = n - x) ==> x <= x'' ==> x'' < n ==> x < n ==> x'' - x < m``)
+          THEN PROVE_TAC[DECIDE ``x <= x'' ==> (x + (x'' - x) = x'')``],
+         PROVE_TAC[L_def]]]);
 
-*)
+val F_ABORT_CLOCK_COMP_ELIM =
+ store_thm
+  ("F_ABORT_CLOCK_COMP_ELIM",
+   ``!M b f. CLOCK_COMP_CORRECT M f
+             ==> CLOCK_COMP_CORRECT M (F_ABORT(f,b))``,
+   RW_TAC arith_ss 
+    [CLOCK_COMP_CORRECT_def,F_SEM_def,UF_SEM,F_CLOCK_COMP_def,
+     F_W_CLOCK_def,F_U_CLOCK_def,PATH_EL_RESTN,L_def,
+     UF_SEM_F_W,UF_SEM_F_G,
+     UF_SEM,B_SEM_def,FIRST_RISE,IS_FINITE_PATH_def,
+     RES_FORALL,RES_EXISTS,PL_def,IN_DEF,NOT_IS_INFINITE_PATH]
+    THEN Cases_on `IS_INFINITE_PATH p`
+    THEN FULL_SIMP_TAC std_ss [NOT_IS_INFINITE_PATH]
+    THEN RW_TAC std_ss []
+    THENL
+     [EQ_TAC
+       THEN RW_TAC std_ss []
+       THENL
+        [PROVE_TAC[],
+         Q.EXISTS_TAC `x`
+          THEN RW_TAC std_ss []
+          THEN Cases_on `UF_SEM M (RESTN p x) (F_CLOCK_COMP (STRONG_CLOCK c) f)`
+          THEN RW_TAC std_ss [IS_FINITE_PATH_RESTN]
+          THEN `0 < x'-x` by DECIDE_TAC
+          THEN `x + (x'-x) = x'` by DECIDE_TAC
+          THEN `x + ((x'-x) - 1) = x' - 1` by DECIDE_TAC
+          THEN Q.EXISTS_TAC `x'-x`
+          THEN RW_TAC arith_ss [PATH_SEG_RESTN]
+          THEN FULL_SIMP_TAC arith_ss [IS_FINITE_PATH_RESTN,intLib.COOPER_PROVE``(!j. ~(j < x''))=(x''=0)``]
+          THEN PROVE_TAC[],
+         PROVE_TAC[],
+         Q.EXISTS_TAC `x`
+          THEN RW_TAC std_ss []
+          THEN Cases_on `UF_SEM M (RESTN p x) (F_CLOCK_COMP (STRONG_CLOCK c) f)`
+          THEN RW_TAC arith_ss [IS_FINITE_PATH_RESTN,intLib.COOPER_PROVE``(!j. ~(j < x''))=(x''=0)``]
+          THEN `x < x + x'` by DECIDE_TAC
+          THEN FULL_SIMP_TAC arith_ss [PATH_SEG_RESTN]
+          THEN PROVE_TAC[DECIDE``(x+x') - 1 = x + x' - 1``]],
+      EQ_TAC
+       THEN RW_TAC std_ss []
+       THENL
+        [PROVE_TAC[],
+         Q.EXISTS_TAC `x`
+          THEN RW_TAC std_ss []
+          THEN Cases_on `UF_SEM M (RESTN p x) (F_CLOCK_COMP (STRONG_CLOCK c) f)`
+          THEN RW_TAC std_ss [IS_FINITE_PATH_RESTN]
+          THEN `PATH_LENGTH (RESTN p x) = PATH_LENGTH p - x` by PROVE_TAC[PATH_LENGTH_RESTN]
+          THEN `PATH_LENGTH (RESTN p x') = PATH_LENGTH p - x'` by PROVE_TAC[PATH_LENGTH_RESTN]
+          THEN FULL_SIMP_TAC arith_ss [IS_FINITE_PATH_RESTN,intLib.COOPER_PROVE``(!j. ~(j < x''))=(x''=0)``]
+          THEN `IS_FINITE_PATH p ==> 0 < PATH_LENGTH (RESTN p x')` by RW_TAC arith_ss []
+          THEN `x'-x < PATH_LENGTH (RESTN p x)` by DECIDE_TAC
+          THEN `0 < x'-x` by DECIDE_TAC
+          THEN `x + (x'-x) = x'` by DECIDE_TAC
+          THEN `x + ((x'-x) - 1) = x' - 1` by DECIDE_TAC
+          THEN Q.EXISTS_TAC `x'-x`
+          THEN RW_TAC arith_ss [PATH_SEG_RESTN]
+          THEN PROVE_TAC[],
+         `!j. j < x ==> ~B_SEM M (getL M (PATH_EL p j)) c` by RW_TAC arith_ss []
+          THEN PROVE_TAC[],
+         `!j. j < x ==> ~B_SEM M (getL M (PATH_EL p j)) c` by RW_TAC arith_ss []
+          THEN Q.EXISTS_TAC `x`
+          THEN RW_TAC std_ss []
+          THEN Cases_on `UF_SEM M (RESTN p x) (F_CLOCK_COMP (STRONG_CLOCK c) f)`
+          THEN RW_TAC arith_ss [IS_FINITE_PATH_RESTN,intLib.COOPER_PROVE``(!j. ~(j < x''))=(x''=0)``]
+          THEN FULL_SIMP_TAC std_ss [IS_FINITE_PATH_RESTN]
+          THEN `PATH_LENGTH (RESTN p x) = PATH_LENGTH p - x` by PROVE_TAC[PATH_LENGTH_RESTN]
+          THEN `x' < PATH_LENGTH (RESTN p x)` by PROVE_TAC[]
+          THEN `x + x' < PATH_LENGTH p` by DECIDE_TAC
+          THEN `x < x + x'` by DECIDE_TAC
+          THEN FULL_SIMP_TAC arith_ss [PATH_SEG_RESTN]
+          THEN RW_TAC arith_ss [FINITE_PATH_NONEMPTY,IS_FINITE_PATH_RESTN]
+          THEN PROVE_TAC[]],
+      EQ_TAC
+       THEN RW_TAC std_ss []
+       THENL
+        [Cases_on `!x. ~B_SEM M (getL M (PATH_EL p x)) c`
+          THEN RW_TAC std_ss []
+          THEN FULL_SIMP_TAC std_ss [NOT_FORALL_THM]
+          THEN ASSUM_LIST
+                (fn thl => ASSUME_TAC(SIMP_RULE std_ss [] (Q.ISPEC `\x. ^(concl(el 1 thl))` WOP)))
+          THEN `?n. B_SEM M (getL M (PATH_EL p n)) c /\
+                    !m. m < n ==> ~B_SEM M (getL M (PATH_EL p m)) c`
+               by PROVE_TAC[]
+          THEN Q.EXISTS_TAC `n`
+          THEN RW_TAC std_ss [RESTN_RESTN,IS_FINITE_PATH_RESTN,PATH_SEG_RESTN]
+          THEN Cases_on `UF_SEM M (RESTN p n) (F_CLOCK_COMP (WEAK_CLOCK c) f)`
+          THEN RW_TAC std_ss []
+          THEN FULL_SIMP_TAC arith_ss 
+                [IS_FINITE_PATH_RESTN,intLib.COOPER_PROVE``(!j. ~(j < x''))=(x''=0)``]
+          THEN ASSUM_LIST(fn thl => FULL_SIMP_TAC std_ss [el 7 thl])
+          THEN `?x''. n < x'' /\
+                      ?p'. (B_SEM M (getL M (PATH_EL p x'')) c /\
+                            B_SEM M (getL M (PATH_EL p x'')) b) /\
+                           UF_SEM M (PATH_CAT (PATH_SEG p (n,x'' - 1),p'))
+                            (F_CLOCK_COMP (WEAK_CLOCK c) f)` by PROVE_TAC[]
+          THEN `0 < x'' - n` by DECIDE_TAC
+          THEN `(n + (x'' -n) = x'') /\ (n + ((x'' - n) - 1) = x'' - 1)` by DECIDE_TAC
+          THEN Q.EXISTS_TAC `x''-n`
+          THEN RW_TAC std_ss [IS_FINITE_PATH_RESTN,PATH_SEG_RESTN]
+          THEN PROVE_TAC[],
+         Cases_on `x' < x` 
+          THEN Cases_on `x < x'`
+          THEN RW_TAC std_ss []
+          THEN RES_TAC
+          THEN `x = x'` by DECIDE_TAC
+          THEN RW_TAC std_ss [],
+         Cases_on `UF_SEM M (RESTN p x'') (F_CLOCK_COMP (WEAK_CLOCK c) f)`
+          THEN RW_TAC arith_ss [IS_FINITE_PATH_RESTN,intLib.COOPER_PROVE``(!j. ~(j < x''))=(x''=0)``]
+          THEN Cases_on `x'' < x` 
+          THEN Cases_on `x < x''`
+          THEN RW_TAC std_ss []
+          THEN RES_TAC
+          THEN `x = x''` by DECIDE_TAC
+          THEN RW_TAC std_ss []
+          THEN Q.EXISTS_TAC `x+x'`
+          THEN RW_TAC arith_ss []
+          THEN FULL_SIMP_TAC arith_ss [PATH_SEG_RESTN]
+          THEN `x + (x' - 1) = x + x' - 1` by DECIDE_TAC
+          THEN PROVE_TAC[],
+         PROVE_TAC[]],
+      EQ_TAC
+       THEN RW_TAC std_ss []
+       THENL
+        [Cases_on `!x. x < PATH_LENGTH p ==> ~B_SEM M (getL M (PATH_EL p x)) c`
+          THEN RW_TAC std_ss []
+          THEN FULL_SIMP_TAC std_ss [NOT_FORALL_THM]
+
+          THEN ASSUM_LIST
+                (fn thl => ASSUME_TAC
+                            (SIMP_RULE std_ss [] 
+                              (Q.ISPEC `\x. ^(concl(el 2 thl)) /\ ^(concl(el 1 thl))` WOP)))
+          THEN `?n. n < PATH_LENGTH p /\ B_SEM M (getL M (PATH_EL p n)) c /\
+                    !m. m < PATH_LENGTH p ==> m < n ==> ~B_SEM M (getL M (PATH_EL p m)) c`
+               by PROVE_TAC[]
+          THEN Q.EXISTS_TAC `n`
+          THEN RW_TAC std_ss [RESTN_RESTN,IS_FINITE_PATH_RESTN,PATH_SEG_RESTN]
+          THEN FULL_SIMP_TAC arith_ss 
+                [IS_FINITE_PATH_RESTN,intLib.COOPER_PROVE``(!j. ~(j < x''))=(x''=0)``]
+          THEN Cases_on `UF_SEM M (RESTN p n) (F_CLOCK_COMP (WEAK_CLOCK c) f)`
+          THEN RW_TAC std_ss []
+          THEN ASSUM_LIST(fn thl => FULL_SIMP_TAC std_ss [el 9 thl] THEN ASSUME_TAC(el 9 thl))
+          THEN `!j. j < n ==> j < PATH_LENGTH p` by DECIDE_TAC
+          THEN `!j. j < n ==> ~B_SEM M (getL M (PATH_EL p j)) c`
+                by PROVE_TAC[]
+          THEN `!x. 0 < PATH_LENGTH(RESTN p x)` by PROVE_TAC[IS_FINITE_PATH_RESTN,FINITE_PATH_NONEMPTY]
+          THEN POP_ASSUM(fn th => FULL_SIMP_TAC std_ss [th])
+          THEN ASSUM_LIST
+                (fn thl => 
+                  STRIP_ASSUME_TAC(SIMP_RULE std_ss (map(fn n=>el n thl)[1,4,6,7]) (Q.SPEC `n` (el 11 thl))))
+          THEN `PATH_LENGTH (RESTN p n) = PATH_LENGTH p - n` by PROVE_TAC[PATH_LENGTH_RESTN]
+          THEN `x'' - n < PATH_LENGTH (RESTN p n) /\ 0 < x'' - n` by RW_TAC arith_ss []
+          THEN Q.EXISTS_TAC `x'' - n`
+          THEN RW_TAC arith_ss []
+          THEN PROVE_TAC[],
+         Cases_on `x' < x` 
+          THEN Cases_on `x < x'`
+          THEN RW_TAC std_ss []
+          THEN RES_TAC
+          THEN `x = x'` by DECIDE_TAC
+          THEN PROVE_TAC[]
+          THEN RW_TAC std_ss [],
+         Cases_on `UF_SEM M (RESTN p x'') (F_CLOCK_COMP (WEAK_CLOCK c) f)`
+          THEN RW_TAC arith_ss [IS_FINITE_PATH_RESTN,intLib.COOPER_PROVE``(!j. ~(j < x''))=(x''=0)``]
+          THEN Cases_on `x'' < x` 
+          THEN Cases_on `x < x''`
+          THEN RW_TAC std_ss []
+          THEN RES_TAC
+          THEN `x = x''` by DECIDE_TAC
+          THEN RW_TAC std_ss []
+          THEN FULL_SIMP_TAC arith_ss [PATH_SEG_RESTN,IS_FINITE_PATH_RESTN]
+          THEN RW_TAC std_ss []
+          THEN `x' < PATH_LENGTH (RESTN p x)` by PROVE_TAC[]
+          THEN `PATH_LENGTH (RESTN p x) = PATH_LENGTH p - x` by PROVE_TAC[PATH_LENGTH_RESTN]
+          THEN `x + x' < PATH_LENGTH p` by DECIDE_TAC
+          THEN `x < x + x'` by DECIDE_TAC
+          THEN Q.EXISTS_TAC `x+x'`
+          THEN RW_TAC arith_ss []
+          THEN `x + (x' - 1) = x + x' - 1` by DECIDE_TAC
+          THEN PROVE_TAC[],
+         PROVE_TAC[]]]);
+
+val F_STRONG_IMP_STRONG_CLOCK_COMP_ELIM =
+ store_thm
+  ("F_STRONG_IMP_STRONG_CLOCK_COMP_ELIM",
+   ``!M r1 r2 p c. 
+      F_SEM M p (STRONG_CLOCK c) (F_STRONG_IMP(r1,r2)) = 
+       UF_SEM M p (F_CLOCK_COMP (STRONG_CLOCK c) (F_STRONG_IMP(r1,r2)))``,
+   RW_TAC arith_ss 
+    [F_SEM_def,UF_SEM,F_CLOCK_COMP_def,
+     F_W_CLOCK_def,F_U_CLOCK_def,PATH_EL_RESTN,L_def,
+     UF_SEM_F_W,UF_SEM_F_G,
+     UF_SEM,B_SEM_def,FIRST_RISE,IS_FINITE_PATH_def,
+     RES_FORALL,RES_EXISTS,PL_def,IN_DEF,NOT_IS_INFINITE_PATH]
+    THEN Cases_on `IS_INFINITE_PATH p`
+    THEN FULL_SIMP_TAC std_ss [NOT_IS_INFINITE_PATH]
+    THEN RW_TAC arith_ss [IS_FINITE_PATH_RESTN,PATH_SEG_RESTN,GSYM S_CLOCK_COMP_ELIM]
+    THENL
+     [EQ_TAC
+       THEN RW_TAC std_ss []
+       THENL
+        [Q.EXISTS_TAC `x`
+          THEN RW_TAC std_ss []
+          THEN `x <= x + x'` by DECIDE_TAC
+          THEN RES_TAC
+          THEN `x' <= x''' - x` by DECIDE_TAC
+          THEN `x + (x''' - x) = x'''` by DECIDE_TAC
+          THEN PROVE_TAC[],
+         Q.EXISTS_TAC `x`
+          THEN RW_TAC std_ss []
+          THEN `x + (x' - x) = x'` by DECIDE_TAC
+          THEN ASSUM_LIST(fn thl => 
+                           STRIP_ASSUME_TAC
+                             (SIMP_RULE arith_ss [el 1 thl, el 2 thl] (Q.SPEC `x'-x` (el 5 thl))))
+          THEN PROVE_TAC[]],
+      EQ_TAC
+       THEN RW_TAC std_ss []
+       THENL
+        [`!x'. x' < PATH_LENGTH p ==> x' < x ==> ~B_SEM M (getL M (PATH_EL p x')) c`
+           by PROVE_TAC[DECIDE``x' < x ==> x < PATH_LENGTH p ==> x' < PATH_LENGTH p``]
+          THEN Q.EXISTS_TAC `x`
+          THEN RW_TAC std_ss []
+          THEN `PATH_LENGTH (RESTN p x) = PATH_LENGTH p - x` by PROVE_TAC[PATH_LENGTH_RESTN]
+          THEN `x+x' < PATH_LENGTH p` by DECIDE_TAC
+          THEN `x <= x+x'` by DECIDE_TAC
+          THEN ASSUM_LIST(fn thl => 
+                           STRIP_ASSUME_TAC
+                             (SIMP_RULE arith_ss [el 2 thl,el 4 thl] (Q.SPEC `x+x'` (el 7 thl))))
+          THEN `x'' - x < PATH_LENGTH (RESTN p x)` by DECIDE_TAC
+          THEN `x' <= x'' - x` by DECIDE_TAC
+          THEN `x + (x'' - x) = x''` by DECIDE_TAC
+          THEN Q.EXISTS_TAC `x'' - x`
+          THEN RW_TAC std_ss [],
+         `!j. j < x ==> ~B_SEM M (getL M (PATH_EL p j)) c` 
+               by PROVE_TAC[DECIDE``j < x ==> x < PATH_LENGTH p ==> j < PATH_LENGTH p``]
+          THEN Q.EXISTS_TAC `x`
+          THEN RW_TAC std_ss []
+          THEN `PATH_LENGTH (RESTN p x) = PATH_LENGTH p - x` by PROVE_TAC[PATH_LENGTH_RESTN]
+          THEN `x' - x < PATH_LENGTH (RESTN p x)` by DECIDE_TAC
+          THEN `x + (x' - x) = x'` by DECIDE_TAC
+          THEN ASSUM_LIST(fn thl => 
+                           STRIP_ASSUME_TAC
+                             (SIMP_RULE arith_ss [el 1 thl, el 2 thl,el 4 thl] (Q.SPEC `x'-x` (el 9 thl))))
+          THEN `x + x'' < PATH_LENGTH p /\ x' <= x + x''` by DECIDE_TAC
+          THEN PROVE_TAC[]]]);
+
+val F_WEAK_IMP_WEAK_CLOCK_COMP_ELIM =
+ store_thm
+  ("F_WEAK_IMP_WEAK_CLOCK_COMP_ELIM",
+   ``!M r1 r2 p c. 
+      F_SEM M p (WEAK_CLOCK c) (F_WEAK_IMP(r1,r2)) = 
+       UF_SEM M p (F_CLOCK_COMP (WEAK_CLOCK c) (F_WEAK_IMP(r1,r2)))``,
+   RW_TAC arith_ss 
+    [F_SEM_def,UF_SEM,F_CLOCK_COMP_def,
+     F_W_CLOCK_def,F_U_CLOCK_def,PATH_EL_RESTN,L_def,
+     UF_SEM_F_W,UF_SEM_F_G,LHAT_def,
+     UF_SEM,B_SEM_def,FIRST_RISE,IS_FINITE_PATH_def,
+     RES_FORALL,RES_EXISTS,PL_def,IN_DEF,NOT_IS_INFINITE_PATH]
+    THEN Cases_on `IS_INFINITE_PATH p`
+    THEN FULL_SIMP_TAC std_ss [NOT_IS_INFINITE_PATH]
+    THEN RW_TAC arith_ss [IS_FINITE_PATH_RESTN,PATH_SEG_RESTN,GSYM S_CLOCK_COMP_ELIM]
+    THENL
+     [EQ_TAC
+       THEN RW_TAC std_ss []
+       THENL
+        [Cases_on `!x. ~B_SEM M (getL M (PATH_EL p x)) c` 
+          THEN RW_TAC std_ss []
+          THEN FULL_SIMP_TAC std_ss [NOT_FORALL_THM]
+          THEN ASSUM_LIST
+                (fn thl => ASSUME_TAC(SIMP_RULE std_ss [] (Q.ISPEC `\x. ^(concl(el 1 thl))` WOP)))
+          THEN `?n. B_SEM M (getL M (PATH_EL p n)) c /\
+                    !m. m < n ==> ~B_SEM M (getL M (PATH_EL p m)) c`
+               by PROVE_TAC[]
+          THEN Q.EXISTS_TAC `n`
+          THEN RW_TAC std_ss [RESTN_RESTN,IS_FINITE_PATH_RESTN,PATH_SEG_RESTN,LHAT_def]
+          THEN Cases_on `(?x''. x' <= x'' /\ S_SEM M (MAP (getL M) (PATH_SEG p (n + x',n + x''))) c r2)`
+          THEN RW_TAC std_ss []
+          THEN FULL_SIMP_TAC arith_ss [NOT_FORALL_THM]
+          THEN ASSUM_LIST
+                (fn thl => ASSUME_TAC(SIMP_RULE std_ss [el 4 thl,el 5 thl] (Q.SPEC `n` (el 8 thl))))
+          THEN ASSUM_LIST
+                (fn thl => STRIP_ASSUME_TAC(SIMP_RULE arith_ss [el 4 thl ] (Q.SPEC `n+x'` (el 1 thl))))
+          THENL
+           [`x' <= x''' - n` by DECIDE_TAC
+             THEN `n + (x''' - n) = x'''` by DECIDE_TAC
+             THEN PROVE_TAC[],
+            `n + x' <= n + x''` by DECIDE_TAC
+             THEN PROVE_TAC[]],
+         Cases_on `!x'''. x'' <= x''' ==>
+                          ?w. S_SEM M (MAP (getL M) (PATH_SEG p (x'',x''')) <> w) c r2`
+          THEN RW_TAC std_ss []
+          THEN FULL_SIMP_TAC std_ss [NOT_FORALL_THM]
+          THEN Cases_on `x' < x` 
+          THEN Cases_on `x < x'`
+          THEN RW_TAC std_ss []
+          THEN RES_TAC
+          THEN `x = x'` by DECIDE_TAC
+          THEN RW_TAC std_ss []
+          THEN POP_ASSUM(K ALL_TAC) THEN POP_ASSUM(K ALL_TAC)
+          THEN `x + (x'' - x) = x''` by DECIDE_TAC
+          THEN ASSUM_LIST
+                (fn thl => STRIP_ASSUME_TAC(SIMP_RULE arith_ss [el 1 thl,el 4 thl] (Q.SPEC `x'' - x` (el 9 thl))))
+          THENL
+           [`x'' <= x + x''''` by DECIDE_TAC
+             THEN PROVE_TAC[],
+            `x'' <= x + (x''' - x)` by DECIDE_TAC
+             THEN `x + (x''' - x) = x'''` by DECIDE_TAC
+             THEN PROVE_TAC[]],
+         PROVE_TAC[]],
+      EQ_TAC
+       THEN RW_TAC std_ss []
+       THENL
+        [Cases_on `!x. x < PATH_LENGTH p ==> ~B_SEM M (getL M (PATH_EL p x)) c` 
+          THEN RW_TAC std_ss []
+          THEN FULL_SIMP_TAC std_ss [NOT_FORALL_THM]
+          THEN ASSUM_LIST
+                (fn thl => ASSUME_TAC
+                            (SIMP_RULE std_ss [] 
+                              (Q.ISPEC `\x. ^(concl(el 2 thl)) /\ ^(concl(el 1 thl))` WOP)))
+          THEN `?n. n < PATH_LENGTH p /\ B_SEM M (getL M (PATH_EL p n)) c /\
+                    !m. m < PATH_LENGTH p ==> m < n ==> ~B_SEM M (getL M (PATH_EL p m)) c`
+               by PROVE_TAC[]
+          THEN Q.EXISTS_TAC `n`
+          THEN RW_TAC std_ss [RESTN_RESTN,IS_FINITE_PATH_RESTN,PATH_SEG_RESTN]
+          THEN Cases_on 
+                `?x''. x'' < PATH_LENGTH (RESTN p n) /\ x' <= x'' /\
+                       S_SEM M (MAP (getL M) (PATH_SEG p (n + x',n + x''))) c r2`
+          THEN RW_TAC std_ss []
+          THEN FULL_SIMP_TAC arith_ss [NOT_EXISTS_THM]
+          THEN `!j. j < n ==> j < PATH_LENGTH p` by DECIDE_TAC
+          THEN `!j. j < n ==> ~B_SEM M (getL M (PATH_EL p j)) c` by PROVE_TAC[]
+          THEN ASSUM_LIST
+                (fn thl => ASSUME_TAC(SIMP_RULE std_ss [el 1 thl,el 9 thl,el 10 thl] (Q.SPEC `n` (el 14 thl))))
+          THEN `PATH_LENGTH (RESTN p n) = PATH_LENGTH p - n` by PROVE_TAC[PATH_LENGTH_RESTN]
+          THEN `n + x' < PATH_LENGTH p` by RW_TAC arith_ss []
+          THEN ASSUM_LIST
+                (fn thl => STRIP_ASSUME_TAC(SIMP_RULE arith_ss [el 1 thl,el 9 thl] (Q.SPEC `n+x'` (el 3 thl))))
+          THENL
+           [`x''' - n < PATH_LENGTH (RESTN p n)` by RW_TAC arith_ss []
+             THEN `x' <= x''' - n` by RW_TAC arith_ss []
+             THEN `n + (x''' - n) = x'''` by RW_TAC arith_ss []
+             THEN PROVE_TAC[],
+            `n + x' <= n + x''` by RW_TAC arith_ss []
+             THEN `n + x'' < PATH_LENGTH p` by RW_TAC arith_ss []
+             THEN PROVE_TAC[]],
+         Cases_on `!x'''. x''' < PATH_LENGTH p ==>
+                          x'' <= x''' ==>
+                          ?w. S_SEM M (MAP (getL M) (PATH_SEG p (x'',x''')) <> w) c r2`
+          THEN RW_TAC std_ss []
+          THEN FULL_SIMP_TAC std_ss [NOT_FORALL_THM]
+          THEN Cases_on `x' < x` 
+          THEN Cases_on `x < x'`
+          THEN RW_TAC std_ss []
+          THEN RES_TAC
+          THEN `x = x'` by DECIDE_TAC
+          THEN RW_TAC std_ss []
+          THEN POP_ASSUM(K ALL_TAC) THEN POP_ASSUM(K ALL_TAC)
+          THEN POP_ASSUM(K ALL_TAC) THEN POP_ASSUM(K ALL_TAC)
+          THEN POP_ASSUM(K ALL_TAC) THEN POP_ASSUM(K ALL_TAC)
+          THEN `x + (x'' - x) = x''` by RW_TAC arith_ss []
+          THEN `PATH_LENGTH (RESTN p x) = PATH_LENGTH p - x` by PROVE_TAC[PATH_LENGTH_RESTN]
+          THEN `x'' - x < PATH_LENGTH (RESTN p x)` by RW_TAC arith_ss []
+          THEN ASSUM_LIST
+                (fn thl => STRIP_ASSUME_TAC
+                             (SIMP_RULE arith_ss [el 1 thl,el 3 thl,el 7 thl] 
+                               (Q.SPEC `x'' - x` (el 14 thl))))
+          THENL
+           [`x'' <= x + x''''` by RW_TAC arith_ss []
+             THEN `x + x'''' < PATH_LENGTH p` by RW_TAC arith_ss []
+             THEN PROVE_TAC[],
+            `x'' <= x + (x''' - x)` by RW_TAC arith_ss []
+             THEN `x''' - x < PATH_LENGTH (RESTN p x)` by RW_TAC arith_ss []
+             THEN `x + (x''' - x) = x'''` by RW_TAC arith_ss []
+             THEN PROVE_TAC[]],
+         PROVE_TAC[]]]);
+
+(******************************************************************************
+* Lemma suggested by Cindy Eisner
+*
+*  p |=clk! {r1} |-> {r2}
+*  <=>
+*  p |= ({r1} |-> {r2}! @clk!) | (({r1} |-> {r2} @ clk) & GF clk)
+******************************************************************************)
+
+val F_WEAK_IMP_STRONG_CLOCK_INFINITE_LEMMA =
+ prove
+  (``!M r1 r2 p c. 
+      IS_INFINITE_PATH p
+      ==>
+      (F_SEM M p (STRONG_CLOCK c) (F_WEAK_IMP(r1,r2)) = 
+        UF_SEM M p
+         (F_OR
+          (F_CLOCK_COMP (STRONG_CLOCK c) (F_STRONG_IMP(r1,r2)),
+           F_AND
+            (F_CLOCK_COMP (WEAK_CLOCK c) (F_WEAK_IMP(r1,r2)),
+             F_G(F_F(F_BOOL c))))))``,
+   ONCE_REWRITE_TAC[F_SEM_def]
+    THEN REWRITE_TAC [F_WEAK_IMP_WEAK_CLOCK_COMP_ELIM,F_STRONG_IMP_STRONG_CLOCK_COMP_ELIM]
+    THEN RW_TAC arith_ss 
+          [UF_SEM,F_CLOCK_COMP_def,PATH_SEG_RESTN,NEXT_RISE_LESS,
+           F_W_CLOCK_def,F_U_CLOCK_def,PATH_EL_RESTN,L_def,
+           UF_SEM_F_W,UF_SEM_F_G,UF_SEM_F_F,LHAT_def,
+           UF_SEM,B_SEM_def,FIRST_RISE,IS_FINITE_PATH_def,
+           RES_FORALL,RES_EXISTS,PL_def,IN_DEF,NOT_IS_INFINITE_PATH,
+           UF_SEM_F_OR]
+    THEN FULL_SIMP_TAC std_ss [NOT_IS_INFINITE_PATH]
+    THEN RW_TAC arith_ss [IS_FINITE_PATH_RESTN,PATH_SEG_RESTN,GSYM S_CLOCK_COMP_ELIM]
+    THEN EQ_TAC
+    THEN RW_TAC std_ss []
+    THENL
+     [PROVE_TAC[],
+      Cases_on
+      `(?x.
+          (B_SEM M (getL M (PATH_EL p x)) c /\
+           !x'.
+             S_SEM M (MAP (getL M) (PATH_SEG p (x,x + x'))) c r1 ==>
+             ?x''.
+               x' <= x'' /\
+               S_SEM M (MAP (getL M) (PATH_SEG p (x + x',x + x''))) c r2) /\
+          !x'. x' < x ==> ~B_SEM M (getL M (PATH_EL p x')) c)`
+       THEN RW_TAC std_ss []
+       THEN FULL_SIMP_TAC std_ss [NOT_EXISTS_THM]
+       THENL
+        [Cases_on `!x. ~B_SEM M (getL M (PATH_EL p x)) c`
+          THEN RW_TAC std_ss []
+          THEN FULL_SIMP_TAC std_ss [NOT_FORALL_THM]
+          THEN Q.EXISTS_TAC `x`
+          THEN RW_TAC std_ss [],
+         ASSUM_LIST(fn thl => STRIP_ASSUME_TAC(Q.SPEC `x'` (el 2 thl)))
+          THEN `x' + (x'' - x') = x''` by DECIDE_TAC
+          THEN PROVE_TAC[]],
+      PROVE_TAC[],
+      PROVE_TAC[],
+      Cases_on
+      `(?x.
+          (B_SEM M (getL M (PATH_EL p x)) c /\
+           !x'.
+             S_SEM M (MAP (getL M) (PATH_SEG p (x,x + x'))) c r1 ==>
+             ?x''.
+               x' <= x'' /\
+               S_SEM M (MAP (getL M) (PATH_SEG p (x + x',x + x''))) c r2) /\
+          !x'. x' < x ==> ~B_SEM M (getL M (PATH_EL p x')) c)`
+       THEN RW_TAC std_ss []
+       THEN FULL_SIMP_TAC std_ss [NOT_EXISTS_THM]
+       THENL
+        [Cases_on `!x. ~B_SEM M (getL M (PATH_EL p x)) c`
+          THEN RW_TAC std_ss []
+          THEN FULL_SIMP_TAC std_ss [NOT_FORALL_THM]
+          THEN Q.EXISTS_TAC `x`
+          THEN RW_TAC std_ss [],
+         ASSUM_LIST(fn thl => STRIP_ASSUME_TAC(Q.SPEC `x'` (el 2 thl)))
+          THEN ASSUM_LIST
+                (fn thl => ASSUME_TAC(SIMP_RULE std_ss [] (Q.ISPEC `\x''. ^(concl(el 1 thl))` WOP)))
+          THEN `?n. B_SEM M (getL M (PATH_EL p (x' + n))) c /\
+                    !m. m < n ==> ~B_SEM M (getL M (PATH_EL p (x' + m))) c`
+               by PROVE_TAC[]
+          THEN Q.EXISTS_TAC `x'+n`
+          THEN RW_TAC arith_ss []
+          THEN `x' + (k - x') = k` by DECIDE_TAC
+          THEN `(k - x') < n` by DECIDE_TAC
+          THEN PROVE_TAC[]],
+      PROVE_TAC[]]);
+
+val F_WEAK_IMP_STRONG_CLOCK_FINITE_LEMMA =
+ prove
+  (``!M r1 r2 p c. 
+      IS_FINITE_PATH p
+      ==>
+      (F_SEM M p (STRONG_CLOCK c) (F_WEAK_IMP(r1,r2)) = 
+        UF_SEM M p
+         (F_OR
+          (F_CLOCK_COMP (STRONG_CLOCK c) (F_STRONG_IMP(r1,r2)),
+           F_AND
+            (F_CLOCK_COMP (WEAK_CLOCK c) (F_WEAK_IMP(r1,r2)),
+             F_G(F_F(F_BOOL c))))))``,
+   ONCE_REWRITE_TAC[F_SEM_def]
+    THEN REWRITE_TAC [F_WEAK_IMP_WEAK_CLOCK_COMP_ELIM,F_STRONG_IMP_STRONG_CLOCK_COMP_ELIM]
+    THEN RW_TAC arith_ss 
+          [UF_SEM,F_CLOCK_COMP_def,PATH_SEG_RESTN,NEXT_RISE_LESS,
+           F_W_CLOCK_def,F_U_CLOCK_def,PATH_EL_RESTN,L_def,
+           UF_SEM_F_W,UF_SEM_F_G,UF_SEM_F_F,LHAT_def,
+           UF_SEM,B_SEM_def,FIRST_RISE,IS_FINITE_PATH_def,
+           RES_FORALL,RES_EXISTS,PL_def,IN_DEF,NOT_IS_INFINITE_PATH,
+           UF_SEM_F_OR]
+    THEN RW_TAC arith_ss [IS_FINITE_PATH_RESTN,PATH_SEG_RESTN,GSYM S_CLOCK_COMP_ELIM]
+    THEN EQ_TAC
+    THEN RW_TAC std_ss []
+    THENL
+     [DISJ1_TAC 
+       THEN Q.EXISTS_TAC `x`
+       THEN PROVE_TAC[],
+      Cases_on
+      `(?x. x < PATH_LENGTH p /\
+            (B_SEM M (getL M (PATH_EL p x)) c /\
+             !x'.
+               x' < PATH_LENGTH (RESTN p x) ==>
+               S_SEM M (MAP (getL M) (PATH_SEG p (x,x + x'))) c r1 ==>
+               ?x''.
+                 x'' < PATH_LENGTH (RESTN p x) /\ x' <= x'' /\
+                 S_SEM M (MAP (getL M) (PATH_SEG p (x + x',x + x''))) c r2) /\
+            !x'.
+              x' < PATH_LENGTH p ==>
+              x' < x ==>
+              ~B_SEM M (getL M (PATH_EL p x')) c)`
+       THEN RW_TAC std_ss []
+       THEN FULL_SIMP_TAC std_ss [NOT_EXISTS_THM]
+       THENL
+        [Cases_on `!x. x < PATH_LENGTH p ==> ~B_SEM M (getL M (PATH_EL p x)) c`
+          THEN RW_TAC std_ss []
+          THEN FULL_SIMP_TAC std_ss [NOT_FORALL_THM]
+          THEN Q.EXISTS_TAC `x`
+          THEN RW_TAC std_ss [],
+         ASSUM_LIST(fn thl => STRIP_ASSUME_TAC(SIMP_RULE std_ss [el 7 thl] (Q.SPEC `x'` (el 3 thl))))
+          THEN RES_TAC
+          THEN `x' + (x'' - x') = x''` by DECIDE_TAC
+          THEN Q.EXISTS_TAC `x'' - x'`
+          THEN RW_TAC arith_ss [PATH_LENGTH_RESTN]],
+      PROVE_TAC[],
+      DISJ1_TAC
+       THEN Q.EXISTS_TAC `x`
+       THEN PROVE_TAC[],
+      Cases_on
+       `(?x. x < PATH_LENGTH p /\
+             (B_SEM M (getL M (PATH_EL p x)) c /\
+              !x'.
+                x' < PATH_LENGTH (RESTN p x) ==>
+                S_SEM M (MAP (getL M) (PATH_SEG p (x,x + x'))) c r1 ==>
+                ?x''.
+                  x'' < PATH_LENGTH (RESTN p x) /\ x' <= x'' /\
+                  S_SEM M (MAP (getL M) (PATH_SEG p (x + x',x + x''))) c r2) /\
+             !x'.
+               x' < PATH_LENGTH p ==>
+               x' < x ==>
+               ~B_SEM M (getL M (PATH_EL p x')) c)`
+       THEN RW_TAC std_ss []
+       THEN FULL_SIMP_TAC std_ss [NOT_EXISTS_THM]
+       THENL
+        [Cases_on `!x. x < PATH_LENGTH p ==> ~B_SEM M (getL M (PATH_EL p x)) c`
+          THEN RW_TAC std_ss []
+          THEN FULL_SIMP_TAC std_ss [NOT_FORALL_THM]
+          THEN Q.EXISTS_TAC `x`
+          THEN RW_TAC std_ss [],
+         ASSUM_LIST(fn thl => STRIP_ASSUME_TAC(Q.SPEC `x'` (el 3 thl)))
+          THEN ASSUM_LIST(fn thl => STRIP_ASSUME_TAC(MATCH_MP (el 1 thl) (el 2 thl)))
+          THEN ASSUM_LIST
+                (fn thl => ASSUME_TAC(SIMP_RULE std_ss [] (Q.ISPEC `\x''. ^(concl(el 2 thl)) /\ ^(concl(el 1 thl))` WOP)))
+          THEN `?n. (n < PATH_LENGTH (RESTN p x') /\
+                    B_SEM M (getL M (PATH_EL p (x' + n))) c) /\
+                    !m. m < n ==>
+                        m < PATH_LENGTH (RESTN p x') ==>
+                        ~B_SEM M (getL M (PATH_EL p (x' + m))) c`
+               by PROVE_TAC[]
+          THEN `PATH_LENGTH(RESTN p x') = PATH_LENGTH p - x'` by PROVE_TAC[PATH_LENGTH_RESTN]
+          THEN `n + x' < PATH_LENGTH p` by DECIDE_TAC
+          THEN Q.EXISTS_TAC `x'+n`
+          THEN RW_TAC arith_ss []
+          THEN `x' + (k - x') = k` by DECIDE_TAC
+          THEN `(k - x') < n` by DECIDE_TAC
+          THEN `(k - x') < PATH_LENGTH (RESTN p x')` by DECIDE_TAC
+          THEN PROVE_TAC[]],
+      DISJ2_TAC
+       THEN RW_TAC std_ss []
+       THEN `PATH_LENGTH (RESTN p x) = PATH_LENGTH p - x` by PROVE_TAC[PATH_LENGTH_RESTN]
+       THEN RES_TAC
+       THEN Q.EXISTS_TAC `x + x'`
+       THEN RW_TAC arith_ss [PATH_LENGTH_RESTN]]);
+
+val F_WEAK_IMP_STRONG_CLOCK_LEMMA =
+ store_thm
+  ("F_WEAK_IMP_STRONG_CLOCK_LEMMA",
+   ``!M r1 r2 p c. 
+      F_SEM M p (STRONG_CLOCK c) (F_WEAK_IMP(r1,r2)) = 
+       UF_SEM M p
+        (F_OR
+         (F_CLOCK_COMP (STRONG_CLOCK c) (F_STRONG_IMP(r1,r2)),
+          F_AND
+           (F_CLOCK_COMP (WEAK_CLOCK c) (F_WEAK_IMP(r1,r2)),
+            F_G(F_F(F_BOOL c)))))``,
+   REPEAT GEN_TAC
+    THEN Cases_on `IS_FINITE_PATH p`
+    THEN PROVE_TAC
+          [NOT_IS_INFINITE_PATH,
+           F_WEAK_IMP_STRONG_CLOCK_INFINITE_LEMMA,
+           F_WEAK_IMP_STRONG_CLOCK_FINITE_LEMMA]);
+
+(******************************************************************************
+* Another lemma suggested by Cindy Eisner
+*
+*  p |= ({r1} |-> {r2}! @clk!) | (({r1} |-> {r2} @ clk) & GF clk)
+*  <=>
+*  p |= ([clk! U (clk & ({r1@clk} |-> {r2@clk}! |
+*                        ((GF clk) & {r1@clk} |-> {r2@clk})))])
+******************************************************************************)
+
+val UF_WEAK_IMP_STRONG_CLOCK_LEMMA =
+ store_thm
+  ("UF_WEAK_IMP_STRONG_CLOCK_LEMMA",
+   ``!M r1 r2 p c. 
+       UF_SEM M p
+        (F_OR
+         (F_CLOCK_COMP (STRONG_CLOCK c) (F_STRONG_IMP(r1,r2)),
+          F_AND
+           (F_CLOCK_COMP (WEAK_CLOCK c) (F_WEAK_IMP(r1,r2)),
+            F_G(F_F(F_BOOL c))))) =
+       UF_SEM M p
+        (F_U_CLOCK c (F_OR
+                      (F_STRONG_IMP(S_CLOCK_COMP c r1, S_CLOCK_COMP c r2),
+                       F_AND
+                        (F_G(F_F(F_BOOL c)),
+                         F_WEAK_IMP(S_CLOCK_COMP c r1, S_CLOCK_COMP c r2)))))``,
+   ONCE_REWRITE_TAC[F_SEM_def]
+    THEN REWRITE_TAC [F_WEAK_IMP_WEAK_CLOCK_COMP_ELIM,F_STRONG_IMP_STRONG_CLOCK_COMP_ELIM]
+    THEN RW_TAC arith_ss 
+          [UF_SEM,F_CLOCK_COMP_def,PATH_SEG_RESTN,NEXT_RISE_LESS,
+           F_W_CLOCK_def,F_U_CLOCK_def,PATH_EL_RESTN,L_def,
+           UF_SEM_F_W,UF_SEM_F_G,UF_SEM_F_F,LHAT_def,
+           UF_SEM,B_SEM_def,FIRST_RISE,IS_FINITE_PATH_def,
+           RES_FORALL,RES_EXISTS,PL_def,IN_DEF,NOT_IS_INFINITE_PATH,
+           UF_SEM_F_OR]
+    THEN Cases_on `IS_INFINITE_PATH p`
+    THEN FULL_SIMP_TAC std_ss [NOT_IS_INFINITE_PATH]
+    THEN RW_TAC arith_ss [IS_FINITE_PATH_RESTN,PATH_SEG_RESTN,GSYM S_CLOCK_COMP_ELIM]
+    THENL
+     [EQ_TAC
+       THEN RW_TAC std_ss []
+       THENL
+        [PROVE_TAC[],
+         Q.EXISTS_TAC `x`
+          THEN RW_TAC std_ss []
+          THEN Cases_on 
+                `(!x'. S_SEM M (MAP (getL M) (PATH_SEG p (x,x + x'))) c r1 ==>
+                       ?x''.
+                         x' <= x'' /\
+                         S_SEM M (MAP (getL M) (PATH_SEG p (x + x',x + x''))) c r2)`
+          THEN RW_TAC std_ss []
+          THEN FULL_SIMP_TAC std_ss [NOT_FORALL_THM]
+          THEN ASSUM_LIST(fn thl => STRIP_ASSUME_TAC(Q.SPEC `x + x'` (el 3 thl)))
+          THEN `x + x' + x''' = x + (x' + x''')` by DECIDE_TAC
+          THEN PROVE_TAC[],
+         PROVE_TAC[],
+         PROVE_TAC[],
+         Cases_on
+          `(?x. (B_SEM M (getL M (PATH_EL p x)) c /\
+                !x'.
+                  S_SEM M (MAP (getL M) (PATH_SEG p (x,x + x'))) c r1 ==>
+                  ?x''.
+                    x' <= x'' /\
+                    S_SEM M (MAP (getL M) (PATH_SEG p (x + x',x + x''))) c r2) /\
+               !x'. x' < x ==> ~B_SEM M (getL M (PATH_EL p x')) c)`
+          THEN RW_TAC std_ss []
+          THEN FULL_SIMP_TAC std_ss [NOT_EXISTS_THM]
+          THENL
+           [Cases_on `!x. ~B_SEM M (getL M (PATH_EL p x)) c`
+             THEN RW_TAC std_ss []
+             THEN FULL_SIMP_TAC std_ss [NOT_FORALL_THM]
+             THEN Q.EXISTS_TAC `x`
+             THEN RW_TAC std_ss [],
+            ASSUM_LIST(fn thl => STRIP_ASSUME_TAC(Q.SPEC `x'` (el 4 thl)))
+             THEN `x + (x' + x'') = x' + (x + x'')` by DECIDE_TAC
+             THEN PROVE_TAC[]]],
+      EQ_TAC
+       THEN RW_TAC std_ss []
+       THENL
+        [Q.EXISTS_TAC `x`
+          THEN RW_TAC std_ss [],
+         Q.EXISTS_TAC `x`
+          THEN RW_TAC std_ss []
+          THEN Cases_on 
+                `(!x'. x' < PATH_LENGTH (RESTN p x) ==>
+                       S_SEM M (MAP (getL M) (PATH_SEG p (x,x + x'))) c r1 ==>
+                       ?x''.
+                         x'' < PATH_LENGTH (RESTN p x) /\ x' <= x'' /\
+                         S_SEM M (MAP (getL M) (PATH_SEG p (x + x',x + x''))) c r2)`
+          THEN RW_TAC std_ss [RESTN_RESTN]
+          THEN FULL_SIMP_TAC std_ss [NOT_FORALL_THM]
+          THEN `PATH_LENGTH (RESTN p x) = PATH_LENGTH p - x`  by PROVE_TAC[PATH_LENGTH_RESTN]
+          THEN `x + x' < PATH_LENGTH p` by DECIDE_TAC
+          THEN `PATH_LENGTH (RESTN p (x + x')) = PATH_LENGTH p - (x + x')`  by PROVE_TAC[PATH_LENGTH_RESTN]
+          THEN ASSUM_LIST(fn thl => STRIP_ASSUME_TAC(Q.SPEC `x + x'` (el 8 thl)))
+          THEN ASSUM_LIST(fn thl => STRIP_ASSUME_TAC(MATCH_MP (el 1 thl) (el 3 thl)))
+          THEN `x + x' + x''' = x + (x' + x''')` by DECIDE_TAC
+          THEN PROVE_TAC[],
+
+         ASSUM_LIST(fn thl => (STRIP_ASSUME_TAC(SIMP_RULE arith_ss [] (Q.SPEC `0` (el 1 thl)))))
+          THEN `?x'. x' < PATH_LENGTH(RESTN p 0) /\ B_SEM M (getL M (PATH_EL p x')) c`
+               by ZAP_TAC arith_ss [FINITE_PATH_NONEMPTY,PATH_LENGTH_RESTN]
+          THEN `PATH_LENGTH (RESTN p 0) =  PATH_LENGTH p` 
+               by RW_TAC arith_ss [PATH_LENGTH_RESTN,FINITE_PATH_NONEMPTY]
+          THEN PROVE_TAC[],
+         DISJ1_TAC
+          THEN Q.EXISTS_TAC `x`
+          THEN RW_TAC std_ss [],
+         Cases_on
+          `(?x. x < PATH_LENGTH p /\
+                (B_SEM M (getL M (PATH_EL p x)) c /\
+                 !x'.
+                   x' < PATH_LENGTH (RESTN p x) ==>
+                   S_SEM M (MAP (getL M) (PATH_SEG p (x,x + x'))) c r1 ==>
+                   ?x''.
+                     x'' < PATH_LENGTH (RESTN p x) /\ x' <= x'' /\
+                     S_SEM M (MAP (getL M) (PATH_SEG p (x + x',x + x''))) c r2) /\
+                !x'.
+                  x' < PATH_LENGTH p ==>
+                  x' < x ==>
+                  ~B_SEM M (getL M (PATH_EL p x')) c)`
+          THEN RW_TAC std_ss []
+          THEN FULL_SIMP_TAC std_ss [NOT_EXISTS_THM]
+          THENL
+           [Cases_on `!x. x < PATH_LENGTH p ==> ~B_SEM M (getL M (PATH_EL p x)) c`
+             THEN RW_TAC std_ss []
+             THEN FULL_SIMP_TAC std_ss [NOT_FORALL_THM]
+             THEN Q.EXISTS_TAC `x`
+             THEN RW_TAC std_ss [],
+            Cases_on `x' < x` 
+             THENL
+              [ASSUM_LIST(fn thl => STRIP_ASSUME_TAC(Q.SPEC `0` (el 6 thl)))
+                THEN FULL_SIMP_TAC arith_ss [RESTN_RESTN]
+                THEN `?x''. x'' < PATH_LENGTH (RESTN p x) /\ B_SEM M (getL M (PATH_EL p (x + x''))) c`
+                     by PROVE_TAC[FINITE_PATH_NONEMPTY,IS_FINITE_PATH_RESTN]
+                THEN `PATH_LENGTH (RESTN p x) = PATH_LENGTH p - x`  by PROVE_TAC[PATH_LENGTH_RESTN]
+                THEN `x' + (x-x') = x` by DECIDE_TAC
+                THEN Q.EXISTS_TAC `x-x'`
+                THEN RW_TAC arith_ss [FINITE_PATH_NONEMPTY,IS_FINITE_PATH_RESTN]
+                THEN `PATH_LENGTH (RESTN p x') = PATH_LENGTH p - x'`  by PROVE_TAC[PATH_LENGTH_RESTN]
+                THEN RW_TAC arith_ss [],
+               ASSUM_LIST(fn thl => STRIP_ASSUME_TAC(Q.SPEC `x'-x` (el 6 thl)))
+                THEN `PATH_LENGTH (RESTN p x) = PATH_LENGTH p - x`  by PROVE_TAC[PATH_LENGTH_RESTN]
+                THEN `x' - x < PATH_LENGTH (RESTN p x)` by DECIDE_TAC
+                THEN ASSUM_LIST
+                      (fn thl => (STRIP_ASSUME_TAC(SIMP_RULE arith_ss [el 1 thl ] (el 3 thl))))
+                THEN `x + (x' - x + x'') = x' + x''` by DECIDE_TAC
+                THEN Q.EXISTS_TAC `x''`
+                THEN ZAP_TAC std_ss []
+                THEN FULL_SIMP_TAC arith_ss [RESTN_RESTN]]]]]);
+
+val F_WEAK_IMP_STRONG_CLOCK_COMP_ELIM =
+ store_thm
+  ("F_WEAK_IMP_STRONG_CLOCK_COMP_ELIM",
+   ``!M r1 r2 p c. 
+       F_SEM M p (STRONG_CLOCK c) (F_WEAK_IMP(r1,r2)) = 
+        UF_SEM M p (F_CLOCK_COMP (STRONG_CLOCK c) (F_WEAK_IMP(r1,r2)))``,
+  PROVE_TAC[F_WEAK_IMP_STRONG_CLOCK_LEMMA, 
+            UF_WEAK_IMP_STRONG_CLOCK_LEMMA,
+            F_CLOCK_COMP_def]);
+
+
+val F_WEAK_IMP_CLOCK_COMP_ELIM =
+ store_thm
+  ("F_WEAK_IMP_CLOCK_COMP_ELIM",
+   ``!M r1 r2. CLOCK_COMP_CORRECT M (F_WEAK_IMP(r1,r2))``,
+   RW_TAC arith_ss 
+    [CLOCK_COMP_CORRECT_def,F_WEAK_IMP_STRONG_CLOCK_COMP_ELIM,
+     F_WEAK_IMP_WEAK_CLOCK_COMP_ELIM]);
+
+val F_STRONG_IMP_WEAK_CLOCK_COMP_ELIM =
+ store_thm
+  ("F_STRONG_IMP_WEAK_CLOCK_COMP_ELIM",
+   ``!M r1 r2 p c. 
+       F_SEM M p (WEAK_CLOCK c) (F_STRONG_IMP(r1,r2)) = 
+        UF_SEM M p (F_CLOCK_COMP (WEAK_CLOCK c) (F_STRONG_IMP(r1,r2)))``,
+   ONCE_REWRITE_TAC[F_SEM_def]
+    THEN REWRITE_TAC [F_WEAK_IMP_WEAK_CLOCK_COMP_ELIM,F_STRONG_IMP_STRONG_CLOCK_COMP_ELIM]
+    THEN RW_TAC (arith_ss++resd)
+          [F_SEM_def,UF_SEM,F_CLOCK_COMP_def,
+           F_W_CLOCK_def,F_U_CLOCK_def,PATH_EL_RESTN,L_def,
+           UF_SEM_F_W,UF_SEM_F_G,UF_SEM_F_F,LHAT_def,
+           UF_SEM,B_SEM_def,FIRST_RISE,IS_FINITE_PATH_def,
+           NOT_IS_INFINITE_PATH,UF_SEM_F_OR,IS_FINITE_PATH_RESTN,
+           PATH_EL_RESTN,IN_DEF,PL_def,
+           intLib.COOPER_PROVE``(!j. ~(j < i)) = (i=0)``]
+    THEN Cases_on `IS_INFINITE_PATH p`
+    THEN FULL_SIMP_TAC std_ss [NOT_IS_INFINITE_PATH]
+    THEN RW_TAC arith_ss [IS_FINITE_PATH_RESTN,PATH_SEG_RESTN,GSYM S_CLOCK_COMP_ELIM]
+    THENL
+     [EQ_TAC
+       THEN RW_TAC std_ss []
+       THENL
+        [PROVE_TAC[],
+         Cases_on `!i. ~B_SEM M (getL M (PATH_EL p i)) c`
+          THEN RW_TAC std_ss []
+          THEN FULL_SIMP_TAC std_ss [NOT_FORALL_THM]
+          THEN Q.EXISTS_TAC `k`
+          THEN RW_TAC std_ss []
+          THEN Cases_on `?i. !i'. ~B_SEM M (getL M (PATH_EL p (i + (i' + k)))) c`
+          THEN RW_TAC std_ss []
+          THEN FULL_SIMP_TAC std_ss [NOT_EXISTS_THM]
+          THEN RES_TAC
+          THENL
+           [PROVE_TAC[],
+            ASSUM_LIST(fn thl => STRIP_ASSUME_TAC(Q.SPEC `k'` (el 3 thl)))
+             THEN ASSUM_LIST
+                   (fn thl => STRIP_ASSUME_TAC(Q.SPEC `k' + (i' + k)` (el 6 thl)))
+             THEN PROVE_TAC[DECIDE``k' + (i' + k) >= k'``]],
+         PROVE_TAC[],
+         PROVE_TAC[],
+         Cases_on
+          `(?k. (B_SEM M (getL M (PATH_EL p k)) c /\
+             !j.
+              S_SEM M (MAP (getL M) (PATH_SEG p (k,j + k))) c r1 ==>
+              ?k'.
+                j <= k' /\
+                S_SEM M (MAP (getL M) (PATH_SEG p (j + k,k + k'))) c r2) /\
+           !j. j < k ==> ~B_SEM M (getL M (PATH_EL p j)) c)`
+          THEN RW_TAC std_ss []
+          THENL
+           [Cases_on `!i. ~B_SEM M (getL M (PATH_EL p i)) c`
+             THEN RW_TAC std_ss []
+             THEN FULL_SIMP_TAC std_ss [NOT_FORALL_THM,NOT_EXISTS_THM]
+             THEN Q.EXISTS_TAC `k`
+             THEN RW_TAC std_ss [],
+            FULL_SIMP_TAC std_ss [NOT_EXISTS_THM]
+             THEN Q.EXISTS_TAC `i+k`
+             THEN PROVE_TAC[intLib.COOPER_PROVE``l >= i + k ==> ?i'. l = i + (i' + k)``]],
+         PROVE_TAC[]],
+      EQ_TAC
+       THEN RW_TAC std_ss []
+       THENL
+        [DISJ1_TAC
+          THEN Q.EXISTS_TAC `k`
+          THEN RW_TAC std_ss [],
+         Cases_on `!i. i < PATH_LENGTH p ==> ~B_SEM M (getL M (PATH_EL p i)) c`
+          THEN RW_TAC std_ss []
+          THEN FULL_SIMP_TAC std_ss [NOT_FORALL_THM]
+          THEN Q.EXISTS_TAC `k`
+          THEN RW_TAC std_ss []
+          THEN Cases_on
+                `?i. i < PATH_LENGTH (RESTN p k) /\
+                  !i'.
+                    i' < PATH_LENGTH (RESTN (RESTN p k) i) ==>
+                    ~B_SEM M (getL M (PATH_EL p (i + (i' + k)))) c`
+          THEN RW_TAC std_ss []
+          THEN FULL_SIMP_TAC std_ss [NOT_EXISTS_THM]
+          THEN RES_TAC
+          THENL
+           [`PATH_LENGTH (RESTN p k) = PATH_LENGTH p - k`
+              by RW_TAC std_ss [PATH_LENGTH_RESTN]
+              THEN `k'' < PATH_LENGTH (RESTN p k)` by DECIDE_TAC
+              THEN Q.EXISTS_TAC `k''`
+              THEN RW_TAC std_ss [],
+            FULL_SIMP_TAC arith_ss [RESTN_RESTN]
+             THEN `PATH_LENGTH (RESTN p k) = PATH_LENGTH p - k` 
+                   by RW_TAC std_ss [PATH_LENGTH_RESTN]
+             THEN `0 < PATH_LENGTH (RESTN p k)`
+                  by RW_TAC std_ss [FINITE_PATH_NONEMPTY,IS_FINITE_PATH_RESTN]
+             THEN `~(k >= k')` by PROVE_TAC[]
+             THEN `k < k'` by DECIDE_TAC
+             THEN `k' - k < PATH_LENGTH (RESTN p k)` by DECIDE_TAC
+             THEN ASSUM_LIST
+                   (fn thl => 
+                    STRIP_ASSUME_TAC(SIMP_RULE std_ss [el 1 thl] (Q.SPEC `k'-k` (el 15 thl))))
+             THEN `k' - k + (i'' + k) = k' + i''` by DECIDE_TAC
+             THEN ASSUM_LIST
+                   (fn thl => STRIP_ASSUME_TAC(Q.SPEC `k' + i''` (el 21 thl)))
+             THEN `k' + i'' >= k'` by DECIDE_TAC
+             THEN `0 < PATH_LENGTH (RESTN p (k' + i''))` 
+                  by RW_TAC std_ss [FINITE_PATH_NONEMPTY,IS_FINITE_PATH_RESTN]
+             THEN ASSUM_LIST
+                   (fn thl => 
+                    STRIP_ASSUME_TAC(SIMP_RULE std_ss [el 1 thl,el 2 thl,el 4 thl] 
+                                                      (LIST_CONJ[el 3 thl,el 5 thl])))
+             THEN `k + (k' - k) = k'` by DECIDE_TAC            
+             THEN ASSUM_LIST
+                   (fn thl => 
+                    STRIP_ASSUME_TAC(SIMP_RULE arith_ss [el 1 thl,RESTN_RESTN] (el 9 thl)))
+             THEN `PATH_LENGTH (RESTN p k') = PATH_LENGTH p - k'` 
+                   by RW_TAC std_ss [PATH_LENGTH_RESTN]
+             THEN `k' + i'' < PATH_LENGTH p` by DECIDE_TAC
+             THEN RES_TAC],
+         DISJ2_TAC
+          THEN RW_TAC arith_ss [],
+         DISJ1_TAC
+          THEN Q.EXISTS_TAC `k`
+          THEN RW_TAC arith_ss [],
+         Cases_on
+          `(?k. k < PATH_LENGTH p /\
+             (B_SEM M (getL M (PATH_EL p k)) c /\
+              !j.
+                j < PATH_LENGTH (RESTN p k) ==>
+                S_SEM M (MAP (getL M) (PATH_SEG p (k,j + k))) c r1 ==>
+                ?k'. k' < PATH_LENGTH (RESTN p k) /\ j <= k' /\
+                     S_SEM M (MAP (getL M) (PATH_SEG p (j + k,k + k'))) c r2) /\
+             !j. j < PATH_LENGTH p ==>
+                 j < k ==>
+                 ~B_SEM M (getL M (PATH_EL p j)) c)`
+          THEN RW_TAC std_ss []
+          THENL
+           [Cases_on`!i. i < PATH_LENGTH p ==> ~B_SEM M (getL M (PATH_EL p i)) c`
+             THEN RW_TAC std_ss []
+             THEN FULL_SIMP_TAC std_ss [NOT_FORALL_THM,NOT_EXISTS_THM]
+             THEN Q.EXISTS_TAC `k`
+             THEN RW_TAC std_ss [],
+            FULL_SIMP_TAC std_ss 
+             [NOT_EXISTS_THM,FINITE_PATH_NONEMPTY,IS_FINITE_PATH_RESTN]
+             THEN `PATH_LENGTH (RESTN p k) = PATH_LENGTH p - k`
+                   by RW_TAC arith_ss [PATH_LENGTH_RESTN]
+             THEN `i + k < PATH_LENGTH p` by DECIDE_TAC
+             THEN Q.EXISTS_TAC `i+k`
+             THEN RW_TAC std_ss []
+             THEN IMP_RES_TAC(intLib.COOPER_PROVE``l >= i + k ==> ?i'. l = i + (i' + k)``)
+             THEN RW_TAC std_ss []
+             THEN `PATH_LENGTH (RESTN (RESTN p k) i) = PATH_LENGTH (RESTN p k) - i`
+                   by RW_TAC arith_ss [PATH_LENGTH_RESTN,IS_FINITE_PATH_RESTN]
+             THEN `i' < PATH_LENGTH (RESTN (RESTN p k) i)` by DECIDE_TAC
+             THEN PROVE_TAC[]],
+         DISJ2_TAC
+          THEN ZAP_TAC std_ss [FINITE_PATH_NONEMPTY]]]);
+
+val F_STRONG_IMP_CLOCK_COMP_ELIM =
+ store_thm
+  ("F_STRONG_IMP_CLOCK_COMP_ELIM",
+   ``!M r1 r2. CLOCK_COMP_CORRECT M (F_STRONG_IMP(r1,r2))``,
+   RW_TAC arith_ss 
+    [CLOCK_COMP_CORRECT_def,F_STRONG_IMP_STRONG_CLOCK_COMP_ELIM,
+     F_STRONG_IMP_WEAK_CLOCK_COMP_ELIM]);
+
+val F_STRONG_CLOCK_CLOCK_COMP_ELIM =
+ store_thm
+  ("F_STRONG_CLOCK_CLOCK_COMP_ELIM",
+   ``!M f. CLOCK_COMP_CORRECT M f
+           ==> !c1. CLOCK_COMP_CORRECT M (F_STRONG_CLOCK(f,c1))``,
+   RW_TAC arith_ss 
+    [CLOCK_COMP_CORRECT_def,F_SEM_def,UF_SEM,F_CLOCK_COMP_def]);
+
+val F_WEAK_CLOCK_CLOCK_COMP_ELIM =
+ store_thm
+  ("F_WEAK_CLOCK_CLOCK_COMP_ELIM",
+   ``!M f. CLOCK_COMP_CORRECT M f
+           ==> !c1. CLOCK_COMP_CORRECT M (F_WEAK_CLOCK(f,c1))``,
+   RW_TAC arith_ss 
+    [CLOCK_COMP_CORRECT_def,F_SEM_def,UF_SEM,F_CLOCK_COMP_def]);
+
+(******************************************************************************
+* EL_AT P m n is true if P is true for the mth time in l at position n
+* (counting from 0 -- so EL_AT P 0 n iff n is the position 
+*  where P is true for the first time)
+******************************************************************************)
+val EL_AT_def =
+ Define
+  `(EL_AT P l 0 n = 
+     n < LENGTH l /\ P(EL n l) /\ !i. i < n ==> ~(P(EL i l)))
+   /\
+   (EL_AT P l (SUC m) n = 
+     n < LENGTH l 
+     /\
+     ?n'. EL_AT P l m n' /\ n' < n /\ P(EL n l) /\ 
+          !i. n' < i /\ i < n ==> ~(P(EL i l)))`;
+
+val EL_AT_0_0 =
+ prove
+  (``P(HD l) ==> (EL_AT P l 0 n = 0 < LENGTH l /\ (n=0))``,
+   RW_TAC arith_ss [EL_AT_def]
+    THEN EQ_TAC
+    THEN RW_TAC arith_ss [EL]
+    THEN Cases_on `n`
+    THEN RW_TAC arith_ss [EL]
+    THEN `0 < SUC n'` by DECIDE_TAC
+    THEN RES_TAC
+    THEN FULL_SIMP_TAC arith_ss [EL]);
+
+val EL_AT_0_SUC =
+ prove
+  (``~(P(HD l)) ==> !n. EL_AT P l 0 n = 0 < n /\ n < LENGTH l /\ EL_AT P (TL l) 0 (n-1)``,
+   RW_TAC list_ss [EL_AT_def,EL]
+    THEN EQ_TAC
+    THEN RW_TAC std_ss []
+    THENL
+     [Cases_on `n=0`
+       THEN FULL_SIMP_TAC list_ss [EL],
+      Cases_on `n=0`
+       THEN FULL_SIMP_TAC list_ss [EL]
+       THEN `0 < LENGTH l` by DECIDE_TAC
+       THEN FULL_SIMP_TAC std_ss [LENGTH_NOT_NULL,NULL_EQ_NIL]
+       THEN `?t h. l = h::t` by PROVE_TAC[list_CASES]
+       THEN RW_TAC list_ss []
+       THEN FULL_SIMP_TAC list_ss [],
+      Cases_on `n=0`
+       THEN FULL_SIMP_TAC list_ss [EL]
+       THEN `0 < LENGTH l` by DECIDE_TAC  
+       THEN `SUC 0 < LENGTH l` by DECIDE_TAC  
+       THEN FULL_SIMP_TAC std_ss [LENGTH_NOT_NULL,NULL_EQ_NIL]
+       THEN `?t h. l = h::t` by PROVE_TAC[list_CASES]
+       THEN RW_TAC list_ss []
+       THEN FULL_SIMP_TAC list_ss [LENGTH]
+       THEN FULL_SIMP_TAC std_ss [LENGTH_NOT_NULL,NULL_EQ_NIL]
+       THEN `?l1 h1. t = h1::l1` by PROVE_TAC[list_CASES]
+       THEN RW_TAC list_ss [],
+      Cases_on `n=0`
+       THEN FULL_SIMP_TAC list_ss [EL]
+       THEN `0 < LENGTH l` by DECIDE_TAC  
+       THEN `SUC 0 < LENGTH l` by DECIDE_TAC  
+       THEN FULL_SIMP_TAC std_ss [LENGTH_NOT_NULL,NULL_EQ_NIL]
+       THEN `?t h. l = h::t` by PROVE_TAC[list_CASES]
+       THEN IMP_RES_TAC(intLib.COOPER_PROVE``~(n = 0) ==> ?m. n = SUC m``)
+       THEN FULL_SIMP_TAC list_ss [EL],
+      Cases_on `n=0`
+       THEN FULL_SIMP_TAC list_ss [EL]
+       THEN `i+1 < n` by DECIDE_TAC
+       THEN RES_TAC
+       THEN FULL_SIMP_TAC list_ss [EL,GSYM ADD1],
+      `n = SUC(n-1)` by DECIDE_TAC
+       THEN PROVE_TAC[EL],
+      Cases_on `i=0`
+       THEN RW_TAC list_ss []
+       THEN `i-1 < n-1` by DECIDE_TAC
+       THEN RES_TAC
+       THEN `i = SUC(i-1)` by DECIDE_TAC
+       THEN PROVE_TAC[EL]]);
+
+val EL_AT_0 =
+ store_thm
+  ("EL_AT_0",
+   ``EL_AT  P l 0 n =
+      if P(HD l) 
+       then 0 < LENGTH l /\ (n=0)
+       else 0 < n /\ n < LENGTH l /\ EL_AT P (TL l) 0 (n-1)``,
+   PROVE_TAC[EL_AT_0_0,EL_AT_0_SUC]);
+
+(******************************************************************************
+* Some properties proved by Michael Norrish
+******************************************************************************)
+local
+
+val ARITH_ss = numSimps.ARITH_ss
+
+val FIRST_EL_AT = prove(
+  ``!l n. EL_AT P l 0 n ==> (EL 0 (FILTER P l) = EL n l)``,
+  CONV_TAC SWAP_VARS_CONV THEN
+  SIMP_TAC (srw_ss()) [EL_AT_def] THEN Induct THENL [
+    SRW_TAC [numSimps.ARITH_ss][] THEN
+    Cases_on `l` THEN
+    FULL_SIMP_TAC (srw_ss() ++ numSimps.ARITH_ss)[listTheory.FILTER],
+
+    SRW_TAC [numSimps.ARITH_ss][] THEN
+    `?h t. l = h :: t` by (Cases_on `l` THEN
+                           FULL_SIMP_TAC (srw_ss() ++ ARITH_ss) []) THEN
+    POP_ASSUM SUBST_ALL_TAC THEN
+    FULL_SIMP_TAC (srw_ss()) [listTheory.FILTER] THEN
+    `~P h` by PROVE_TAC [DECIDE ``0 < SUC n``, listTheory.EL,
+                         listTheory.HD] THEN
+    SRW_TAC [][] THEN FIRST_X_ASSUM MATCH_MP_TAC THEN
+    SRW_TAC [ARITH_ss][] THEN
+    FIRST_X_ASSUM (Q.SPEC_THEN `SUC i` MP_TAC) THEN
+    SRW_TAC [ARITH_ss][]
+  ]);
+
+val EL_AT_LENGTH = prove(
+  ``!n m l. EL_AT P l m n ==> n < LENGTH l``,
+  REPEAT GEN_TAC THEN Cases_on `m` THEN
+  SRW_TAC [ARITH_ss][EL_AT_def]);
+
+val EL_AT_NIL = prove(
+  ``!P n m. ~(EL_AT P [] m n)``,
+  REPEAT STRIP_TAC THEN IMP_RES_TAC EL_AT_LENGTH THEN
+  FULL_SIMP_TAC (srw_ss() ++ ARITH_ss) []);
+
+val NOT_ZERO_LT_ZERO = arithmeticTheory.NOT_ZERO_LT_ZERO
+
+val EL_AT_P_EL = prove(
+  ``!P m n l. EL_AT P l m n ==> P (EL n l)``,
+  GEN_TAC THEN Induct THEN SRW_TAC [][EL_AT_def]);
+
+val EL_AT_CONS = prove(
+  ``!P m t n h. EL_AT P (h::t) m n =
+                   if P h then
+                     (m = 0) /\ (n = 0) \/
+                     0 < m /\ 0 < n /\ EL_AT P t (m - 1) (n - 1)
+                   else
+                     0 < n /\ EL_AT P t m (n - 1)``,
+  GEN_TAC THEN Induct THENL [
+    SRW_TAC [ARITH_ss][EL_AT_def, EQ_IMP_THM] THENL [
+      SPOSE_NOT_THEN ASSUME_TAC THEN
+      `~P (EL 0 (h::t))` by PROVE_TAC [NOT_ZERO_LT_ZERO] THEN
+      FULL_SIMP_TAC (srw_ss()) [],
+      SRW_TAC [][GSYM NOT_ZERO_LT_ZERO] THEN
+      DISCH_THEN SUBST_ALL_TAC THEN FULL_SIMP_TAC (srw_ss()) [],
+      SRW_TAC [][GSYM NOT_ZERO_LT_ZERO] THEN
+      DISCH_THEN ASSUME_TAC THEN
+      `n = 0` by SRW_TAC [ARITH_ss][] THEN FULL_SIMP_TAC (srw_ss()) [],
+      Cases_on `n` THEN FULL_SIMP_TAC (srw_ss() ++ ARITH_ss) [],
+      FIRST_X_ASSUM (Q.SPEC_THEN `SUC i` MP_TAC) THEN
+      SRW_TAC [ARITH_ss][],
+      Cases_on `n` THEN FULL_SIMP_TAC (srw_ss() ++ ARITH_ss) [],
+      Cases_on `i` THEN SRW_TAC [][] THEN
+      FIRST_X_ASSUM MATCH_MP_TAC THEN SRW_TAC [ARITH_ss][]
+    ],
+
+    REPEAT GEN_TAC THEN Cases_on `P h` THEN
+    ASM_SIMP_TAC (srw_ss() ++ ARITH_ss)[EL_AT_def] THENL [
+      SRW_TAC [ARITH_ss][EQ_IMP_THM] THEN SRW_TAC [][] THENL [
+        SRW_TAC [ARITH_ss][EL_AT_def] THENL [
+          Cases_on `n` THEN FULL_SIMP_TAC (srw_ss() ++ ARITH_ss) [],
+          FIRST_X_ASSUM (MP_TAC o SPEC ``SUC i``) THEN
+          SRW_TAC [ARITH_ss][]
+        ],
+        PROVE_TAC [arithmeticTheory.LESS_TRANS],
+        Cases_on `m` THEN FULL_SIMP_TAC (srw_ss() ++ ARITH_ss) [] THEN
+        SRW_TAC [ARITH_ss][EL_AT_def] THEN
+        Q.EXISTS_TAC `n' - 1` THEN SRW_TAC [ARITH_ss][] THENL [
+          Cases_on`n` THEN FULL_SIMP_TAC (srw_ss() ++ ARITH_ss) [],
+          FIRST_X_ASSUM (Q.SPEC_THEN `SUC i` MP_TAC) THEN
+          SRW_TAC [ARITH_ss][]
+        ],
+        `n - 1 < LENGTH t` by PROVE_TAC [EL_AT_LENGTH] THEN
+        SRW_TAC [ARITH_ss][],
+        IMP_RES_TAC EL_AT_P_EL THEN
+        `P (EL n (h :: t))` by
+            (`n = SUC (n - 1)` by DECIDE_TAC THEN
+             POP_ASSUM SUBST1_TAC THEN SRW_TAC [][]) THEN
+        SRW_TAC [][] THEN
+        Cases_on `m` THEN SRW_TAC [ARITH_ss][] THENL [
+          `!i. i < n - 1 ==> ~P(EL i t)` by PROVE_TAC [EL_AT_def] THEN
+          Cases_on `i` THEN FULL_SIMP_TAC (srw_ss() ++ ARITH_ss) [],
+          `n - 1 < LENGTH t /\
+           ?m. EL_AT P t n' m /\ m < n - 1 /\
+               !j. m < j /\ j < n - 1 ==> ~P (EL j t)`
+             by PROVE_TAC [EL_AT_def] THEN
+          Q.EXISTS_TAC `SUC m` THEN
+          SRW_TAC [ARITH_ss][] THEN
+          Cases_on `i` THEN FULL_SIMP_TAC (srw_ss() ++ ARITH_ss) []
+        ]
+      ],
+
+      SRW_TAC [ARITH_ss][EQ_IMP_THM] THEN SRW_TAC [][] THENL [
+        DECIDE_TAC,
+        DECIDE_TAC,
+        Q.EXISTS_TAC `n' - 1` THEN
+        SRW_TAC [ARITH_ss][] THENL [
+          Cases_on `n` THEN FULL_SIMP_TAC (srw_ss() ++ ARITH_ss) [],
+          FIRST_X_ASSUM (Q.SPEC_THEN `SUC i` MP_TAC) THEN
+          SRW_TAC [ARITH_ss][]
+        ],
+        Q.EXISTS_TAC `n' + 1` THEN SRW_TAC [ARITH_ss][] THENL [
+          Cases_on `n` THEN FULL_SIMP_TAC (srw_ss() ++ ARITH_ss) [],
+          Cases_on `i` THEN FULL_SIMP_TAC (srw_ss() ++ ARITH_ss) []
+        ]
+      ]
+    ]
+  ]);
+
+in
+
+val EL_AT_FILTER_LENGTH = prove(
+  ``!l m n. EL_AT P l m n ==> m < LENGTH (FILTER P l)``,
+  Induct THENL [
+    SRW_TAC [][EL_AT_NIL],
+    SRW_TAC [][EL_AT_CONS, listTheory.FILTER] THENL [
+      DECIDE_TAC,
+      PROVE_TAC [DECIDE ``0 < x /\ x - 1 < y ==> x < SUC y``],
+      PROVE_TAC []
+    ]
+  ]);
+
+val EL_AT_FILTER = prove(
+  ``!l m n. EL_AT P l m n ==> (EL m (FILTER P l) = EL n l)``,
+  Induct THEN SRW_TAC [][EL_AT_NIL, EL_AT_CONS, listTheory.FILTER] THENL [
+    SRW_TAC [][],
+    Q.PAT_ASSUM `EL_AT v x y z` MP_TAC THEN
+    Cases_on `m` THEN Cases_on `n` THEN
+    FULL_SIMP_TAC (srw_ss() ++ ARITH_ss) [],
+    Q.PAT_ASSUM `EL_AT v x y z` MP_TAC THEN
+    Cases_on `n` THEN FULL_SIMP_TAC (srw_ss() ++ ARITH_ss) []
+  ]);
+
+end;
+
+(******************************************************************************
+* Ken McMillan's rule for compositional reasoning
+* Not(f2 U f1) And Not(f1 U f2) Implies G(f1 And f2)
+******************************************************************************)
+
+val UF_SEM_NOT_UNTIL_NOT =
+ store_thm
+  ("UF_SEM_NOT_UNTIL_NOT",
+   ``UF_SEM M p (F_NOT(F_UNTIL (f1, F_NOT f2))) =
+      !i :: PL p. (!j. j < i ==> UF_SEM M (RESTN p j) f1) 
+                  ==> UF_SEM M (RESTN p i) f2``,
+   Cases_on `IS_FINITE_PATH p`
+    THEN RW_TAC (arith_ss++resd)
+          [PATH_EL_RESTN,L_def,IS_FINITE_PATH_RESTN,
+           UF_SEM,B_SEM_def,FIRST_RISE,IS_FINITE_PATH_def,
+           PL_def,IN_DEF,NOT_IS_INFINITE_PATH]
+    THEN TRY(PROVE_TAC[])
+    THEN EQ_TAC
+    THEN RW_TAC std_ss []
+    THENL
+     [ASSUM_LIST(fn thl => STRIP_ASSUME_TAC(Q.SPEC `i` (el 3 thl)))
+       THEN PROVE_TAC[],
+      Cases_on `?j. j < PATH_LENGTH p /\ j < k /\ ~UF_SEM M (RESTN p j) f1`
+       THEN RW_TAC std_ss []
+       THEN Cases_on `k < PATH_LENGTH p`
+       THEN RW_TAC std_ss []
+       THEN FULL_SIMP_TAC arith_ss [NOT_EXISTS_THM]
+       THEN `!j. j < k ==> j < PATH_LENGTH p` by RW_TAC arith_ss []
+       THEN PROVE_TAC[]]);
+
+val McMillan_RULE =
+ store_thm
+  ("McMillan_RULE",
+   ``UF_SEM M p (F_NOT(F_UNTIL (f2, F_NOT f1)))
+     /\
+     UF_SEM M p (F_NOT(F_UNTIL (f1, F_NOT f2)))
+     ==>
+     UF_SEM M p (F_G(F_AND(f1,f2)))``,
+   RW_TAC (std_ss++resd) [UF_SEM_NOT_UNTIL_NOT,IN_DEF]
+    THEN SIMP_TAC (std_ss++resd) [UF_SEM_F_G,UF_SEM,IN_DEF]
+    THEN INDUCT_THEN COMPLETE_INDUCTION ASSUME_TAC
+    THEN RW_TAC arith_ss []
+    THEN FULL_SIMP_TAC arith_ss [PL_def]
+    THEN `!m. m < i ==> (IS_FINITE_PATH p ==> m < PATH_LENGTH p)` by RW_TAC arith_ss [PL_def]
+    THEN TRY(PROVE_TAC[])
+    THEN RES_TAC
+    THEN DECIDE_TAC);
+
+(******************************************************************************
+* Formula implication f1 --> f2
+******************************************************************************)
+val F_IMPLIES_def =
+ Define 
+  `F_IMPLIES(f1,f2) = F_OR(F_NOT f1, f2)`;
+
+val UF_SEM_F_IMPLIES =
+ store_thm
+  ("UF_SEM_F_IMPLIES",
+   ``UF_SEM M p (F_IMPLIES (f1,f2)) = UF_SEM M p f1 ==> UF_SEM M p f2``,
+   RW_TAC std_ss [UF_SEM,F_IMPLIES_def,UF_SEM_F_OR]
+    THEN PROVE_TAC[]);
+
+(******************************************************************************
+* Iterate a function
+******************************************************************************)
+val ITER_def =
+ Define
+  `(ITER g 0 x = x) /\ (ITER g (SUC n) x = ITER g n (g x))`;
+
+val ITER_ALT =
+ prove
+  (``!n x. ITER g (SUC n) x = g(ITER g n x)``,
+   Induct
+    THEN PROVE_TAC[ITER_def]);
+
+(******************************************************************************
+* A recursive form of a while-loop with test b and body g
+******************************************************************************)
+val REC_def =
+ Define
+  `REC f b g = !n. f n = if b n then f(g n) else n`;
+
+val REC_ITER_LEMMA1 =
+ prove
+  (``REC f b g 
+     ==> 
+     !n x. (!m. m < n ==> b(ITER g m x)) /\ ~(b(ITER g n x)) ==> (f x = ITER g n x)``,
+   DISCH_TAC
+    THEN Induct
+    THEN RW_TAC arith_ss [ITER_def]
+    THENL
+     [PROVE_TAC[REC_def],
+      ASSUM_LIST(fn thl => ASSUME_TAC(Q.SPEC `g x` (el 3 thl)))
+       THEN `b x` by PROVE_TAC[ITER_def,DECIDE ``0 < SUC m``]
+       THEN `f(g x) = f x` by PROVE_TAC[REC_def]
+       THEN `!m. m < n ==> b (ITER g m (g x))` by ALL_TAC
+       THEN TRY(PROVE_TAC[])
+       THEN RW_TAC arith_ss []
+       THEN `SUC m < SUC n` by DECIDE_TAC
+       THEN PROVE_TAC[ITER_def]]);
+
+val REC_ITER_LEMMA2 =
+ prove
+  (``REC f b g
+     /\
+     (!m. m < n ==> b(seq m) ==> (seq(m+1) = g(seq m))) 
+     /\ 
+     (!m. m < n ==> b(seq m))
+     ==> 
+     (!m. m <= n ==> (seq m = ITER g m (seq 0)))``,
+   STRIP_TAC
+    THEN Induct
+    THEN RW_TAC arith_ss [ITER_def]
+    THEN `m < n` by DECIDE_TAC
+    THEN RES_TAC
+    THEN RES_TAC
+    THEN RW_TAC std_ss [ADD1]
+    THEN `m <= n` by DECIDE_TAC
+    THEN PROVE_TAC[ITER_ALT,ITER_def]);
+
+(******************************************************************************
+* A kind of Hoare logic while-rule.
+* b, g are arbitary functions, and f satisfies:
+*
+*  All x. f x = if b x then f(g x) else x
+*
+* The atomic proposition "s = x" means the state has value x
+*
+*          p |= G((s = x) --> X!(s = g x)
+*     ------------------------------------------
+*       p |= (s = x) --> [b W (!b & (s = f x))]
+*
+******************************************************************************)
+val REC_UNTIL =
+ store_thm
+  ("REC_UNTIL",
+   ``!B R f b g.
+      REC f b g 
+      /\
+      (!n. UF_SEM (SIMPLE_KRIPKE_STRUCTURE B R) p
+            (F_G
+             (F_IMPLIES
+              (F_AND(F_BOOL(B_PROP(\s. s = n)),F_BOOL(B_PROP b)),
+               F_NEXT(F_BOOL(B_PROP(\s. s = g n)))))))
+      ==> 
+      (!n. UF_SEM (SIMPLE_KRIPKE_STRUCTURE B R) p
+            (F_IMPLIES
+              (F_BOOL(B_PROP(\s. s = n)),
+               F_W(F_BOOL(B_PROP b), 
+                   F_AND(F_NOT(F_BOOL(B_PROP b)), 
+                         F_BOOL(B_PROP(\s. s = f n)))))))``,
+   Cases_on `~(IS_FINITE_PATH p)`
+    THEN RW_TAC (arith_ss++resd)
+     [UF_SEM,PATH_EL_RESTN,UF_SEM_F_W,UF_SEM_F_G,IN_DEF,PL_def,L_def,B_SEM_def,
+      UF_SEM_F_IMPLIES,UF_SEM_F_G,IS_FINITE_PATH_RESTN,
+      getL_def,getP_def,SIMPLE_KRIPKE_STRUCTURE_def]
+    THENL
+     [Cases_on `!i. b (PATH_EL p i)`
+       THEN RW_TAC std_ss []
+       THEN FULL_SIMP_TAC std_ss [NOT_FORALL_THM]
+       THEN ASSUM_LIST
+             (fn thl => ASSUME_TAC(SIMP_RULE std_ss [] (Q.ISPEC `\i. ^(concl(el 1 thl))` WOP)))
+       THEN `?n. ~b (PATH_EL p n) /\ !m. m < n ==> b (PATH_EL p m)`
+            by PROVE_TAC[]
+       THEN Q.EXISTS_TAC `n`
+       THEN ASM_SIMP_TAC std_ss []
+       THEN IMP_RES_TAC REC_ITER_LEMMA2
+       THEN `!m. m < n ==> b (ITER g m (PATH_EL p 0))` by PROVE_TAC[DECIDE``m<n ==> m<=n``]
+       THEN `~b (ITER g n (PATH_EL p 0))` by PROVE_TAC[DECIDE``n<=n``]
+       THEN IMP_RES_TAC REC_ITER_LEMMA1
+       THEN PROVE_TAC[DECIDE``m <= m``],
+      RW_TAC std_ss []
+       THEN Cases_on `!i. i < PATH_LENGTH p ==> b (PATH_EL p i)`
+       THEN RW_TAC std_ss []
+       THEN FULL_SIMP_TAC std_ss [NOT_FORALL_THM]
+       THEN ASSUM_LIST
+             (fn thl => ASSUME_TAC(SIMP_RULE std_ss [] 
+                         (Q.ISPEC `\i. ^(concl(el 2 thl)) /\ ^(concl(el 1 thl))` WOP)))
+       THEN `?n. (n < PATH_LENGTH p /\ ~b (PATH_EL p n)) /\
+                 !m. m < n ==> ~(m < PATH_LENGTH p) \/ b (PATH_EL p m)`
+             by PROVE_TAC[]
+       THEN Q.EXISTS_TAC `n`
+       THEN `!m. m < PATH_LENGTH p ==> m < n ==> b (PATH_EL p m)` by PROVE_TAC[]
+       THEN ASM_SIMP_TAC std_ss []
+       THEN `!m. m < n ==> b (PATH_EL p m)` by PROVE_TAC[DECIDE``m < n /\ n < r ==> m < r``]
+       THEN `!m. m < n ==> b (PATH_EL p m) ==> (PATH_EL p (m + 1) = g (PATH_EL p m))` 
+            by PROVE_TAC[DECIDE``m < n /\ n < r ==> m < r``]
+       THEN IMP_RES_TAC REC_ITER_LEMMA2
+       THEN `!m. m < n ==> b (ITER g m (PATH_EL p 0))` by PROVE_TAC[DECIDE``m<n ==> m<=n``]
+       THEN `~b (ITER g n (PATH_EL p 0))` by PROVE_TAC[DECIDE``n<=n``]
+       THEN IMP_RES_TAC REC_ITER_LEMMA1
+       THEN PROVE_TAC[DECIDE``m <= m``]]);
+
+val UF_SEM_NOT_SUFFIX_IMP_FALSE =
+ store_thm
+  ("UF_SEM_NOT_SUFFIX_IMP_FALSE",
+   ``UF_SEM M p (F_NOT (F_SUFFIX_IMP (r,F_BOOL (B_NOT B_TRUE)))) =
+      ?j :: PL p. US_SEM M (LHAT M (PATH_SEG p (0,j))) r``,
+   RW_TAC (arith_ss++resd) 
+    [PATH_EL_RESTN,L_def,IS_FINITE_PATH_RESTN,
+     UF_SEM,B_SEM_def,FIRST_RISE,IS_FINITE_PATH_def,
+     PL_def,IN_DEF,NOT_IS_INFINITE_PATH]);
+
+val UF_SEM_STRONG_IMP_DEF =
+ store_thm
+  ("UF_SEM_STRONG_IMP_DEF",
+   ``UF_SEM M p (F_STRONG_IMP(r1,r2)) =
+     UF_SEM M p 
+      (F_SUFFIX_IMP(r1, F_NOT(F_SUFFIX_IMP(r2, F_BOOL(B_NOT B_TRUE)))))``,
+   RW_TAC (arith_ss++resd) 
+    [PATH_EL_RESTN,L_def,IS_FINITE_PATH_RESTN,
+     UF_SEM,B_SEM_def,FIRST_RISE,IS_FINITE_PATH_def,
+     PL_def,IN_DEF,NOT_IS_INFINITE_PATH,PATH_SEG_RESTN]
+    THEN Cases_on `~(IS_FINITE_PATH p)`
+    THEN RW_TAC std_ss []
+    THENL
+     [EQ_TAC
+       THEN RW_TAC std_ss []
+       THENL
+        [RES_TAC
+          THEN `j + (k-j) = k` by DECIDE_TAC
+          THEN EXISTS_TAC ``k-j``
+          THEN RW_TAC arith_ss [],
+         RES_TAC
+          THEN EXISTS_TAC ``j+j'``
+          THEN RW_TAC arith_ss []],
+      EQ_TAC
+       THEN RW_TAC std_ss []
+       THENL
+        [RES_TAC
+          THEN `PATH_LENGTH (RESTN p j) = PATH_LENGTH p - j` by PROVE_TAC[PATH_LENGTH_RESTN]
+          THEN `j + (k-j) = k` by DECIDE_TAC
+          THEN EXISTS_TAC ``k-j``
+          THEN RW_TAC arith_ss [],
+         RES_TAC
+          THEN `PATH_LENGTH (RESTN p j) = PATH_LENGTH p - j` by PROVE_TAC[PATH_LENGTH_RESTN]
+          THEN EXISTS_TAC ``j+j'``
+          THEN RW_TAC arith_ss []]]);
 
 val _ = export_theory();
-
 
 
 
